-emit_rocq: Soundness proof (#976)
* WIP AxSem

* WIP Soundness proof

* LogicalHeaps WIP

* LogicalHeaps WIP

* WIP LogicalHeaps

* WIP Proved consume, produce soundness

* WIP SymexSoundness

* verify_place_expr_elem_sound

* verify_place_expr_sound

* verify_statement_sound

* verify_call_sound

* verify_ghost_command_sound

* verify_terminator_sound

* verify_basic_blocks_sound

* verify_body

* Fail CI if the Rocq metatheory proofs fail

* alloc_params_sound

* alloc_locals_sound

* alloc_locals_sound: adapt proof to Iris 4.1

I was using Iris 4.3 on my laptop, but CI uses Iris 4.1.

* verify_body_sound

* body_is_correct_sound

* verified_program_has_no_ub

* Cleanup

bin/rust/rocq/SymbolicExecution.v
@@ -1,8 +1,24 @@
-Require Export Annotations.
+Require Export Annotations Values.
 From Coq Require Export ClassicalDescription.
+
+Open Scope annot_scope.
 
 Notation "f @@ x" := (f x)
   (at level 20, right associativity, only parsing).
+
+Fixpoint remove1_assoc{T}(x: string)(xys: list (string * T)): option (T * list (string * T)) :=
+  match xys with
+    [] => None
+  | (x', y')::xys =>
+    if string_dec x' x then
+      Some (y', xys)
+    else
+      match remove1_assoc x xys with
+        None => None
+      | Some (y, xys) =>
+        Some (y, (x', y')::xys)
+      end
+  end.
 
 Fixpoint assoc_{A B}(eq_dec: forall (x1 x2: A), {x1 = x2} + {x1 <> x2})(x: A)(xys: list (A * B)): option B :=
   match xys with
@@ -12,25 +28,6 @@ Fixpoint assoc_{A B}(eq_dec: forall (x1 x2: A), {x1 = x2} + {x1 <> x2})(x: A)(xy
       Some y
     else
       assoc_ eq_dec x xys
-  end.
-
-Fixpoint assoc{T}(x: string)(xys: list (string * T)): option T :=
-  match xys with
-    [] => None
-  | (x', y)::xys =>
-    if string_dec x x' then
-      Some y
-    else
-      assoc x xys
-  end.
-
-Fixpoint combine_{A B}(xs: list A)(ys: list B): list (A * B) * (list A * list B) :=
-  match xs, ys with
-    [], ys => ([], ([], ys))
-  | xs, [] => ([], (xs, []))
-  | (x::xs), (y::ys) =>
-    let '(xys, (xs, ys)) := combine_ xs ys in
-    ((x, y)::xys, (xs, ys))
   end.
 
 Fixpoint nth__iter{T}(k: nat)(xs_done: list T)(xs_todo: list T): option (T * list T) :=
@@ -48,27 +45,21 @@ decide equality.
 apply string_dec.
 Defined.
 
-Parameter Ptr: Set.
+Fixpoint Ty_eq_dec(ty1 ty2: Ty) {struct ty1}: {ty1 = ty2} + {ty1 <> ty2}
+with GenericArg_eq_dec(arg1 arg2: GenericArg) {struct arg1}: {arg1 = arg2} + {arg1 <> arg2}
+with GenericArgList_eq_dec(args1 args2: GenericArgList) {struct args1}: {args1 = args2} + {args1 <> args2}.
+- decide equality.
+  + decide equality.
+  + decide equality.
+  + apply string_dec.
+- decide equality.
+- decide equality.
+Defined.
 
-Parameter null_ptr: Ptr.
-
-Inductive Value :=
-| VPtr(ptr: Ptr)
-| VBool(b: bool)
-| VReal(q: Q)
-| VDummy (* Used as the value of nonsensical expressions *)
-| VSome(v: Value)
-| VTuple0
-.
-
-Definition value_eqb(v1 v2: Value): bool.
-Admitted.
-
-Lemma value_eqb_def_(v1 v2: Value): (VBool (value_eqb v1 v2) = VBool true) = (v1 = v2).
-Admitted.
+Definition Ty_eqb(ty1 ty2: Ty): bool := if Ty_eq_dec ty1 ty2 then true else false.
 
 Inductive LocalState :=
-| LSValue(v: Value)
+| LSValue(v: option Value)
 | LSPlace(a: Ptr) (* The environment records (a pointer to) the place where this local variable's value is stored, not the value itself *)
 .
 
@@ -96,7 +87,7 @@ Definition forall_ty(trace: Trace)(ty: Ty)(Q: Value -> Prop): Prop :=
   end.
 
 Definition havoc(trace: Trace)(x: string)(ty: Ty)(env: Env)(Q: Env -> Value -> Prop): Prop :=
-  forall_ty trace ty @@ fun v => Q ((x, LSValue v)::env) v.
+  forall_ty trace ty @@ fun v => Q ((x, LSValue (Some v))::env) v.
 
 Fixpoint havoc_vars(trace: Trace)(vars: list (string * Ty))(env: Env)(Q: Env -> Prop): Prop :=
   match vars with
@@ -104,16 +95,15 @@ Fixpoint havoc_vars(trace: Trace)(vars: list (string * Ty))(env: Env)(Q: Env -> 
   | (x, ty)::vars => havoc trace x ty env (fun env _ => havoc_vars trace vars env Q)
   end.
 
-Inductive Pred :=
-| PointsTo(ty: Ty)
-| PointsTo_(ty: Ty)
-| UserPred(name: string)
+Inductive PrimChunk :=
+| PointsTo_(ty: Ty)(ptr: Value)(rhs: Value)
 .
 
-Record Chunk := {
-    pred: Pred;
-    args: list Value
-}.
+Inductive Chunk :=
+| Prim(chunk: PrimChunk)
+| PointsTo(ty: Ty)(ptr: Value)(rhs: Value)
+| User(pred_name: string)(args: list Value)
+.
 
 Definition Heap := list Chunk.
 
@@ -124,9 +114,9 @@ Fixpoint eval(env: Env)(e: Expr): Value :=
   | NullPtr => VPtr null_ptr
   | Var x =>
     match assoc x env with
-      Some (LSValue v) => v
+      Some (LSValue (Some v)) => v
     | Some (LSPlace ptr) => VPtr ptr
-    | None => VDummy
+    | _ => VDummy
     end
   | Eq e1 e2 => VBool (value_eqb (eval env e1) (eval env e2))
   end.
@@ -155,7 +145,7 @@ Definition assert(trace: Trace)(env: Env)(e: Expr)(Q: Prop): Prop :=
 Definition produce_pat(trace: Trace)(env: Env)(ty: Ty)(pat: Pat)(Q: Env -> Value -> Prop): Prop :=
   match pat with
     LitPat e => Q env (eval env e)
-  | VarPat x => havoc trace x ty env Q
+  | VarPat x => forall v, Q ((x, LSValue (Some v))::env) v
   end.
 
 Fixpoint produce_pats(trace: Trace)(env: Env)(pats: list Pat)(Q: Env -> list Value -> Prop): Prop :=
@@ -174,11 +164,12 @@ Fixpoint produce(trace: Trace)(h: Heap)(env: Env)(tree: SymexTree)(a: Asn)(Q: He
   match a with
     BoolAsn e => assume env e @@ Q h env tree
   | PointsToAsn ty ptr rhs =>
+    let ptr := eval env ptr in
     produce_pat trace env ty rhs @@ fun env vrhs =>
-    Q ({| pred := PointsTo ty; args := [eval env ptr; vrhs] |}::h) env tree
+    Q (PointsTo ty ptr vrhs::h) env tree
   | PredAsn name args =>
     produce_pats trace env args @@ fun env vs =>
-    Q ({| pred := UserPred name; args := vs |}::h) env tree
+    Q (User name vs::h) env tree
   | SepAsn a1 a2 =>
     produce trace h env tree a1 @@ fun h env tree =>
     produce trace h env tree a2 Q
@@ -194,7 +185,7 @@ Fixpoint produce(trace: Trace)(h: Heap)(env: Env)(tree: SymexTree)(a: Asn)(Q: He
 Definition match_pat(env: Env)(pat: Pat)(v: Value)(Q: Env -> Prop): Prop :=
   match pat with
     LitPat e => v = eval env e /\ Q env
-  | VarPat x => Q ((x, LSValue v)::env)
+  | VarPat x => Q ((x, LSValue (Some v))::env)
   end.
 
 Fixpoint match_pats(trace: Trace)(env: Env)(pats: list Pat)(vs: list Value)(Q: Env -> Prop): Prop :=
@@ -213,8 +204,8 @@ Fixpoint consume_chunk(trace: Trace)(h: Heap)(tree: SymexTree)(Q: Heap -> SymexT
       None => Error trace "consume_chunk: AutoOpen: bad heap index" (k, h)
     | Some (chunk, h) =>
       match chunk with
-        {| pred := PointsTo ty; args := [ptr; v] |} =>
-        let h := {| pred := PointsTo_ ty; args := [ptr; VSome v] |}::h in
+        PointsTo ty ptr v =>
+        let h := Prim (PointsTo_ ty ptr (VSome v))::h in
         consume_chunk trace h tree Q
       | _ => Error trace "consume_chunk: AutoOpen: bad chunk" chunk
       end
@@ -230,22 +221,22 @@ Fixpoint consume_chunk(trace: Trace)(h: Heap)(tree: SymexTree)(Q: Heap -> SymexT
 
 Definition consume_points_to(trace: Trace)(h: Heap)(tree: SymexTree)(ty: Ty)(ptr: Value)(Q: Heap -> SymexTree -> Value -> Prop): Prop :=
   consume_chunk trace h tree @@ fun h tree chunk =>
-  pred chunk = PointsTo ty /\
-  match args chunk with
-    [ptr'; v] =>
+  match chunk with
+    PointsTo ty' ptr' v =>
+    ty' = ty /\
     ptr' = ptr /\
     Q h tree v
-  | _ => Error trace "consume_points_to: bad PointsTo args" (args chunk)
+  | _ => Error trace "consume_points_to: bad chunk" chunk
   end.
 
 Definition consume_points_to_(trace: Trace)(h: Heap)(tree: SymexTree)(ty: Ty)(ptr: Value)(Q: Heap -> SymexTree -> Value -> Prop): Prop :=
   consume_chunk trace h tree @@ fun h tree chunk =>
-  pred chunk = PointsTo_ ty /\
-  match args chunk with
-    [ptr'; v] =>
+  match chunk with
+    Prim (PointsTo_ ty' ptr' v) =>
+    ty' = ty /\
     ptr' = ptr /\
     Q h tree v
-  | _ => Error trace "consume_points_to_: bad PointsTo_ args" (args chunk)
+  | _ => Error trace "consume_points_to_: bad chunk" chunk
   end.
 
 Fixpoint consume(trace: Trace)(h: Heap)(env: Env)(tree: SymexTree)(a: Asn)(Q: Heap -> Env -> SymexTree -> Prop): Prop :=
@@ -257,9 +248,13 @@ Fixpoint consume(trace: Trace)(h: Heap)(env: Env)(tree: SymexTree)(a: Asn)(Q: He
     Q h env tree
   | PredAsn name pats =>
     consume_chunk trace h tree @@ fun h tree chunk =>
-    pred chunk = UserPred name /\
-    match_pats trace env pats (args chunk) @@ fun env =>
-    Q h env tree
+    match chunk with
+      User name' args =>
+      name = name' /\
+      match_pats trace env pats args @@ fun env =>
+      Q h env tree
+    | _ => Error trace "consume: PredAsn: bad chunk" chunk
+    end
   | SepAsn a1 a2 =>
     consume trace h env tree a1 @@ fun h env tree =>
     consume trace h env tree a2 Q
@@ -278,18 +273,46 @@ Variable preds: list (string * PredDef).
 Variable specs: list (string * Spec).
 Variable trees: list (ProofObligation * SymexTree).
 
-Fixpoint process_param_addr_taken_steps(trace: Trace)(h: Heap)(env: Env)(tree: SymexTree)(Q: Heap -> Env -> SymexTree -> Prop): Prop :=
-  match tree with
-    ParamAddrTaken x true;; tree => Error trace "process_param_addr_taken_steps: ParamAddrTaken true is not yet supported" tree
-  | ParamAddrTaken x false;; tree => process_param_addr_taken_steps trace h env tree Q
-  | tree => Q h env tree
+Fixpoint alloc_params(trace: Trace)(h: Heap)(tree: SymexTree)(param_env: list ((Local * LocalDecl) * Value))
+    (Q: Heap -> Env -> SymexTree -> forall (dealloc_params: Trace -> Heap -> Env -> SymexTree -> (Heap -> SymexTree -> Prop) -> Prop), Prop)
+    {struct param_env}
+    : Prop :=
+  match param_env with
+    [] => Q h [] tree (fun trace h env tree Q => Q h tree)
+  | ((x, _), arg)::param_env =>
+    match tree with
+      ParamAddrTaken x' b;; tree =>
+      if string_dec x' x then
+        if b then
+          Error trace "alloc_params: ParamAddrTaken true is not yet supported" tree
+        else
+          alloc_params trace h tree param_env @@ fun h env tree dealloc_params =>
+          let dealloc_params trace h env tree Q :=
+            match remove1_assoc x env with
+            | Some (LSValue _, env) =>
+              dealloc_params trace h env tree Q
+            | remove_result => Error trace "alloc_params: dealloc_params: local not found" (x, env, remove_result)
+            end
+          in
+          let env := (x, LSValue (Some arg))::env in
+          Q h env tree dealloc_params
+      else
+        Error trace "alloc_params: ParamAddrTaken: param name does not match" (x', x)
+    | tree =>
+      Error trace "alloc_params: bad tree: ParamAddrTaken expected" tree
+    end
   end.
 
-Fixpoint process_local_addr_taken_steps(trace: Trace)(h: Heap)(env: Env)(tree: SymexTree)(local_decls: list (Local * LocalDecl))
-    (Q: Heap -> Env -> SymexTree -> forall (dealloc_heapy_locals: Heap -> SymexTree -> (Heap -> SymexTree -> Prop) -> Prop), Prop)
+Fixpoint alloc_locals(trace: Trace)(h: Heap)(env: Env)(tree: SymexTree)(local_decls: list (Local * LocalDecl))
+    (Q: Heap -> Env -> SymexTree -> forall (dealloc_locals: Trace -> Heap -> Env -> SymexTree -> (Heap -> Env -> SymexTree -> Prop) -> Prop), Prop)
+    {struct local_decls}
     : Prop :=
   match local_decls with
-    [] => Q h env tree (fun h tree Q => Q h tree)
+    [] =>
+    let dealloc_locals trace h env tree Q :=
+      Q h env tree
+    in
+    Q h env tree dealloc_locals
   | (x, {| ty := ty |})::local_decls =>
     match tree with
       LocalAddrTaken x' b;; tree =>
@@ -297,22 +320,29 @@ Fixpoint process_local_addr_taken_steps(trace: Trace)(h: Heap)(env: Env)(tree: S
         if b then
           forall ptr value,
           ptr <> null_ptr ->
-          let '(h, cleanup_heapy_locals) :=
-            match ty with
-              Never | Tuple0 => (h, (fun cleanup_heapy_locals' => cleanup_heapy_locals'))
-            | _ =>
-              ({| pred := PointsTo_ ty; args := [VPtr ptr; value] |}::h,
-               (fun cleanup_heapy_locals' h tree Q =>
+          let '(h, dealloc_locals) :=
+            if Ty_eqb ty Never || Ty_eqb ty Tuple0 then
+              (h, (fun dealloc_locals' => dealloc_locals'))
+            else
+              (Prim (PointsTo_ ty (VPtr ptr) value)::h,
+               (fun dealloc_locals' trace h env tree Q =>
                 consume_points_to_ trace h tree ty (VPtr ptr) @@ fun h tree _ =>
-                cleanup_heapy_locals' h tree Q))
-            end
+                dealloc_locals' trace h env tree Q))
           in
           let env := ((x, LSPlace ptr)::env) in
-          process_local_addr_taken_steps trace h env tree local_decls @@ fun h env tree cleanup_heapy_locals' =>
-          Q h env tree (cleanup_heapy_locals cleanup_heapy_locals')
+          alloc_locals trace h env tree local_decls @@ fun h env tree dealloc_locals' =>
+          Q h env tree (dealloc_locals dealloc_locals')
         else
-          let env := ((x, LSValue VDummy)::env) in
-          process_local_addr_taken_steps trace h env tree local_decls Q
+          let env := ((x, LSValue None)::env) in
+          alloc_locals trace h env tree local_decls @@ fun h env tree dealloc_locals' =>
+          let dealloc_locals trace h env tree Q :=
+            match remove1_assoc x env with
+            | Some (LSValue _, env) =>
+              dealloc_locals' trace h env tree Q
+            | remove_result => Error trace "alloc_locals: dealloc_locals: local not found" (x, env, remove_result)
+            end
+          in
+          Q h env tree dealloc_locals
       else
         Error trace "process_local_addr_taken_steps: local variable name does not match" tree
     | _ => Error trace "process_local_addr_taken_steps: bad tree: LocalAddrTaken expected" tree
@@ -325,7 +355,7 @@ Variable local_decls: list (Local * LocalDecl).
 
 Definition load_from_pointer(trace: Trace)(h: Heap)(tree: SymexTree)(ty: Ty)(ptr: Value)(Q: Heap -> SymexTree -> Value -> Prop): Prop :=
   consume_points_to trace h tree ty ptr @@ fun h tree v =>
-  let h := {| pred := PointsTo ty; args := [ptr; v] |}::h in
+  let h := PointsTo ty ptr v::h in
   Q h tree v.
 
 Inductive Place :=
@@ -333,32 +363,35 @@ Inductive Place :=
 | PDeref(ptr: Value)
 .
 
-Definition load_from_place(trace: Trace)(h: Heap)(env: Env)(tree: SymexTree)(place: Place)(ty: Ty)(Q: Heap -> Env -> SymexTree -> Value -> Prop): Prop :=
+Definition load_from_place(trace: Trace)(h: Heap)(env: Env)(tree: SymexTree)(place: Place)(ty: Ty)(Q: Heap -> SymexTree -> Value -> Prop): Prop :=
   match place with
     PNonAddrTakenLocal x =>
     match assoc x env with
-      Some (LSValue v) => Q h env tree v
+      Some (LSValue (Some v)) => Q h tree v
     | _ => Error trace "load_from_place: dangling local" (x, env)
     end
   | PDeref ptr =>
     load_from_pointer trace h tree ty ptr @@ fun h tree v =>
-    Q h env tree v
+    Q h tree v
   end.
 
 Definition store_to_place(trace: Trace)(h: Heap)(env: Env)(tree: SymexTree)(place: Place)(ty: Ty)(v: Value)(Q: Heap -> Env -> SymexTree -> Prop): Prop :=
-  match ty with
-    Tuple0 => Q h env tree
-  | _ =>
+  if Ty_eq_dec ty Tuple0 then
+    Q h env tree
+  else
     match place with
       PNonAddrTakenLocal x =>
-      let env := (x, LSValue v)::env in
-      Q h env tree
+      match remove1_assoc x env with
+      | Some (LSValue _, xys) =>
+        let env := (x, LSValue (Some v))::xys in
+        Q h env tree
+      | _ => Error trace "store_to_place: no such local" (x, env)
+      end
     | PDeref ptr =>
       consume_points_to_ trace h tree ty ptr @@ fun h tree _ =>
-      let h := {| pred := PointsTo ty; args := [ptr; v] |}::h in
+      let h := PointsTo ty ptr v::h in
       Q h env tree
-    end
-  end.
+    end.
 
 Definition verify_local(trace: Trace)(env: Env)(x: Local)(Q: Place -> Ty -> Prop): Prop :=
   match assoc x local_decls with
@@ -369,18 +402,18 @@ Definition verify_local(trace: Trace)(env: Env)(x: Local)(Q: Place -> Ty -> Prop
     | None => Error trace "verify_local: dangling local" (x, env)
     end
   | None => Error trace "verify_local: no such local" x
- end.
+  end.
 
 Definition verify_place_expr_elem
     (trace: Trace)
     (h: Heap)(env: Env)(tree: SymexTree)(place: Place)(ty: Ty)(place_expr_elem: PlaceExprElem)
-    (Q: Heap -> Env -> SymexTree -> Place -> Ty -> Prop)
+    (Q: Heap -> SymexTree -> Place -> Ty -> Prop)
     : Prop :=
   match place_expr_elem with
   | Deref =>
-    load_from_place trace h env tree place ty @@ fun h env tree v =>
+    load_from_place trace h env tree place ty @@ fun h tree v =>
     match ty with
-      RawPtr ty => Q h env tree (PDeref v) ty
+      RawPtr ty => Q h tree (PDeref v) ty
     | _ => Error trace "verify_place_expr_elem: Deref: bad place type: must match RawPtr _" ty
     end
   end.
@@ -388,68 +421,69 @@ Definition verify_place_expr_elem
 Fixpoint verify_place_expr_elems
     (trace: Trace)
     (h: Heap)(env: Env)(tree: SymexTree)(place: Place)(ty: Ty)(place_expr_elems: list PlaceExprElem)
-    (Q: Heap -> Env -> SymexTree -> Place -> Ty -> Prop)
+    (Q: Heap -> SymexTree -> Place -> Ty -> Prop)
+    {struct place_expr_elems}
     : Prop :=
   match place_expr_elems with
-    [] => Q h env tree place ty
+    [] => Q h tree place ty
   | place_expr_elem::place_expr_elems =>
-    verify_place_expr_elem trace h env tree place ty place_expr_elem @@ fun h env tree place ty =>
+    verify_place_expr_elem trace h env tree place ty place_expr_elem @@ fun h tree place ty =>
     verify_place_expr_elems trace h env tree place ty place_expr_elems Q
   end.
 
-Definition verify_place_expr(trace: Trace)(h: Heap)(env: Env)(tree: SymexTree)(place_expr: PlaceExpr)(Q: Heap -> Env -> SymexTree -> Place -> Ty -> Prop): Prop :=
+Definition verify_place_expr(trace: Trace)(h: Heap)(env: Env)(tree: SymexTree)(place_expr: PlaceExpr)(Q: Heap -> SymexTree -> Place -> Ty -> Prop): Prop :=
   let '(x, place_expr_elems) := place_expr in
   verify_local trace env x @@ fun place ty =>
   verify_place_expr_elems trace h env tree place ty place_expr_elems Q.
 
-Definition verify_operand(trace: Trace)(h: Heap)(env: Env)(tree: SymexTree)(operand: Operand)(Q: Heap -> Env -> SymexTree -> Value -> Ty -> Prop): Prop :=
+Definition verify_operand(trace: Trace)(h: Heap)(env: Env)(tree: SymexTree)(operand: Operand)(Q: Heap -> SymexTree -> Value -> Ty -> Prop): Prop :=
   match operand with
     Move place_expr =>
-    verify_place_expr trace h env tree place_expr @@ fun h env tree place ty =>
-    load_from_place trace h env tree place ty @@ fun h env tree v =>
-    Q h env tree v ty
+    verify_place_expr trace h env tree place_expr @@ fun h tree place ty =>
+    load_from_place trace h env tree place ty @@ fun h tree v =>
+    Q h tree v ty
   | Copy place_expr =>
-    verify_place_expr trace h env tree place_expr @@ fun h env tree place ty =>
-    load_from_place trace h env tree place ty @@ fun h env tree v =>
-    Q h env tree v ty
+    verify_place_expr trace h env tree place_expr @@ fun h tree place ty =>
+    load_from_place trace h env tree place ty @@ fun h tree v =>
+    Q h tree v ty
   | Constant (Val ZeroSized Tuple0) =>
-    Q h env tree VTuple0 Tuple0
+    Q h tree VTuple0 Tuple0
   | _ => Error trace "verify_operand: unsupported operand" operand
   end.
 
 Fixpoint verify_operands
     (trace: Trace)(h: Heap)(env: Env)(tree: SymexTree)(operands: list Operand)
-    (Q: Heap -> Env -> SymexTree -> list Value -> Prop)
+    (Q: Heap -> SymexTree -> list Value -> Prop)
     : Prop :=
   match operands with
-    [] => Q h env tree []
+    [] => Q h tree []
   | operand::operands =>
-    verify_operand trace h env tree operand @@ fun h env tree v ty =>
-    verify_operands trace h env tree operands @@ fun h env tree vs =>
-    Q h env tree (v::vs)
+    verify_operand trace h env tree operand @@ fun h tree v ty =>
+    verify_operands trace h env tree operands @@ fun h tree vs =>
+    Q h tree (v::vs)
   end.
 
-Definition verify_rvalue(trace: Trace)(h: Heap)(env: Env)(tree: SymexTree)(rvalue: Rvalue)(Q: Heap -> Env -> SymexTree -> Value -> Ty -> Prop): Prop :=
+Definition verify_rvalue(trace: Trace)(h: Heap)(env: Env)(tree: SymexTree)(rvalue: Rvalue)(Q: Heap -> SymexTree -> Value -> Ty -> Prop): Prop :=
   match rvalue with
     Use operand =>
     verify_operand trace h env tree operand Q
   | RawPtr_ place_expr =>
-    verify_place_expr trace h env tree place_expr @@ fun h env tree place ty =>
+    verify_place_expr trace h env tree place_expr @@ fun h tree place ty =>
     match place with
       PNonAddrTakenLocal _ => Error trace "verify_rvalue: RawPtr_: place must not be PNonAddrTakenLocal" place
-    | PDeref ptr => Q h env tree ptr (RawPtr ty)
+    | PDeref ptr => Q h tree ptr (RawPtr ty)
     end
   | Cast PtrToPtr operand ty =>
-    verify_operand trace h env tree operand @@ fun h env tree v ty0 =>
-    Q h env tree v ty (* We do not support wide pointers yet, so this does not change the value *)
+    verify_operand trace h env tree operand @@ fun h tree v ty0 =>
+    Q h tree v ty (* We do not support wide pointers yet, so this does not change the value *)
   | _ => Error trace "verify_rvalue: unsupported rvalue" rvalue
   end.
 
 Definition verify_statement(trace: Trace)(h: Heap)(env: Env)(tree: SymexTree)(statement: Statement)(Q: Heap -> Env -> SymexTree -> Prop): Prop :=
   match statement with
   | Assign lhs rhs =>
-    verify_rvalue trace h env tree rhs @@ fun h env tree v ty_rhs =>
-    verify_place_expr trace h env tree lhs @@ fun h env tree place ty => (* SOUNDNESS: Is it okay to evaluate the RHS before the LHS? *)
+    verify_rvalue trace h env tree rhs @@ fun h tree v ty_rhs =>
+    verify_place_expr trace h env tree lhs @@ fun h tree place ty => (* SOUNDNESS: Is it okay to evaluate the RHS before the LHS? *)
     store_to_place trace h env tree place ty v Q
   | StorageLive x => Q h env tree (* SOUNDNESS BUG: Ignored for now. https://github.com/verifast/verifast/issues/948 *)
   | StorageDead x => Q h env tree (* SOUNDNESS BUG: Ignored for now. https://github.com/verifast/verifast/issues/948 *)
@@ -479,16 +513,17 @@ Definition assume_value_neq_N(trace: Trace)(v: Value)(ty: Ty)(value: N)(Q: Prop)
   end.
 
 Fixpoint verify_switch_int
-    (trace: Trace)(h: Heap)(env: Env)(tree: SymexTree)(v: Value)(ty: Ty)(values: list N)(targets: list BasicBlock)
-    (Qbb: Heap -> Env -> SymexTree -> BasicBlock -> Prop)
+    (trace: Trace)(tree: SymexTree)(discr: Value)(ty: Ty)(values: list N)(targets: list BasicBlock)
+    (Qbb: SymexTree -> BasicBlock -> Prop)
+    {struct values}
     : Prop :=
   match values, targets with
-    [], [default_target] => Qbb h env tree default_target
+    [], [default_target] => Qbb tree default_target
   | value::values, target::targets =>
     match tree with
       Fork tree1 tree2 =>
-      (assume_value_neq_N trace v ty value @@ verify_switch_int (SecondBranch::trace) h env tree1 v ty values targets Qbb) /\
-      (assume_value_eq_N trace v ty value @@ Qbb h env tree2 target)
+      (assume_value_neq_N trace discr ty value @@ verify_switch_int (SecondBranch::trace) tree1 discr ty values targets Qbb) /\
+      (assume_value_eq_N trace discr ty value @@ Qbb tree2 target)
     | _ => Error trace "verify_switch_int: bad tree: Fork expected" tree
     end
   | _, _ => Error trace "verify_switch_int: length mismatch" (values, targets)
@@ -498,29 +533,27 @@ Definition verify_call
     (trace: Trace)(h: Heap)(tree: SymexTree)(func_name: string)(targs: list GenericArg)(args: list Value)
     (Q: Heap -> SymexTree -> Value -> Prop)
     : Prop :=
-  match func_name with
-    "std::ptr::mut_ptr::<impl *mut T>::is_null" =>
+  if string_dec func_name "std::ptr::mut_ptr::<impl *mut T>::is_null" then
     match args with
       [ptr] =>
       Q h tree (VBool (value_eqb ptr (VPtr null_ptr)))
     | _ =>  Error trace "verify_call: is_null: bad args" args
     end
-  | "std::ptr::null_mut" =>
+  else if string_dec func_name "std::ptr::null_mut" then
     Q h tree (VPtr null_ptr)
-  | "std::process::abort" =>
+  else if string_dec func_name "std::process::abort" then
     True
-  | _ =>
+  else
     match assoc func_name specs with
       None => Error trace "verify_call: callee has no spec" func_name
     | Some spec =>
-      let env := combine (map fst (spec_params spec)) (map LSValue args) in
+      let env := combine (map fst (spec_params spec)) (map (fun v => LSValue (Some v)) args) in
       consume trace h env tree (pre spec) @@ fun h env tree =>
       forall_ty trace (spec_output spec) @@ fun result =>
-      let env := ("result", LSValue result)::env in
+      let env := ("result", LSValue (Some result))::env in
       produce trace h env tree (post spec) @@ fun h env tree =>
       Q h tree result
-    end
-  end.
+    end.
 
 Fixpoint eval_pats(trace: Trace)(env: Env)(pats: list Pat)(Q: list Value -> Prop): Prop :=
   match pats with
@@ -532,30 +565,38 @@ Fixpoint eval_pats(trace: Trace)(env: Env)(pats: list Pat)(Q: list Value -> Prop
   | pat::pats => Error trace "eval_pats: pattern not supported here" pat
   end.
 
-Definition verify_ghost_command(trace: Trace)(h: Heap)(env: Env)(tree: SymexTree)(Q: Heap -> Env -> SymexTree -> Prop): Prop :=
+Definition verify_ghost_command(trace: Trace)(h: Heap)(env: Env)(tree: SymexTree)(Q: Heap -> SymexTree -> Prop): Prop :=
   match tree with
     Open;; tree =>
     consume_chunk trace h tree @@ fun h tree chunk =>
-    match pred chunk with
-      UserPred pred_name =>
+    match chunk with
+      User pred_name args =>
       match assoc pred_name preds with
         None => Error trace "verify_ghost_command: Open: no such predicate" pred_name
       | Some pred_def =>
-        let env' := combine (map fst (params pred_def)) (map LSValue (args chunk)) in
-        produce trace h env' tree (body pred_def) @@ fun h _ tree =>
-        Q h env tree
+        match combine_ (params pred_def) args with
+          (env, ([], [])) =>
+          let env := map (fun '((x, ty), v) => (x, LSValue (Some v))) env in
+          produce trace h env tree (body pred_def) @@ fun h _ tree =>
+          Q h tree
+        | _ => Error trace "verify_ghost_command: Open: bad chunk: has bad argument count" (chunk, pred_def)
+        end
       end
-    | _ => Error trace "verify_ghost_command: Open: predicate not supported" (pred chunk)
+    | _ => Error trace "verify_ghost_command: Open: predicate not supported" chunk
     end
   | Close (RealLit 1%Q) pred_name [] arg_pats;; tree =>
     eval_pats trace env arg_pats @@ fun vs =>
     match assoc pred_name preds with
       None => Error trace "verify_ghost_command: Close: no such predicate" pred_name
     | Some pred_def =>
-      let env' := combine (map fst (params pred_def)) (map LSValue vs) in
-      consume trace h env' tree (body pred_def) @@ fun h _ tree =>
-      let h := {| pred := UserPred pred_name; args := vs |}::h in
-      Q h env tree
+      match combine_ (params pred_def) vs with
+        (env, ([], [])) =>
+        let env := map (fun '((x, ty), v) => (x, LSValue (Some v))) env in
+        consume trace h env tree (body pred_def) @@ fun h _ tree =>
+        let h := User pred_name vs::h in
+        Q h tree
+      | _ => Error trace "verify_ghost_command: Close: bad argument count" (arg_pats, pred_def)
+      end
     end
   | _ => Error trace "verify_ghost_command: bad tree: no ghost command found" tree
   end.
@@ -569,25 +610,27 @@ Definition verify_terminator
   match terminator with
     Goto bb => Qbb h env tree bb
   | SwitchInt discr values targets =>
-    verify_operand trace h env tree discr @@ fun h env tree v ty =>
-    verify_switch_int trace h env tree v ty values targets Qbb
+    verify_operand trace h env tree discr @@ fun h tree v ty =>
+    verify_switch_int trace tree v ty values targets @@ fun tree bb =>
+    Qbb h env tree bb
   | Return => Qreturn h env tree
   | Unreachable => Error trace "verify_terminator: Unreachable: reached" tt
-  | Call ({| func := Constant (Val ZeroSized (FnDef "VeriFast_ghost_command" [])) |} as call) =>
-    verify_ghost_command trace h env tree @@ fun h env tree =>
-    match target call with
-      None => Error trace "verify_terminator: Call: VeriFast_ghost_command: target expected" tt
-    | Some bb => Qbb h env tree bb
-    end
   | Call ({| func := Constant (Val ZeroSized (FnDef name targs)) |} as call) =>
-    verify_operands trace h env tree (VfMir.args call) @@ fun h env tree args =>
-    verify_call trace h tree name targs args @@ fun h tree result =>
-    verify_place_expr trace h env tree (destination call) @@ fun h env tree place ty =>
-    store_to_place trace h env tree place ty result @@ fun h env tree =>
-    match target call with
-      None => Error trace "verify_terminator: Call: target expected" tt
-    | Some bb => Qbb h env tree bb
-    end
+    if string_dec name "VeriFast_ghost_command" then
+      verify_ghost_command trace h env tree @@ fun h tree =>
+      match target call with
+        None => Error trace "verify_terminator: Call: VeriFast_ghost_command: target expected" tt
+      | Some bb => Qbb h env tree bb
+      end
+    else
+      verify_operands trace h env tree (VfMir.args call) @@ fun h tree args =>
+      verify_call trace h tree name (list_of_GenericArgList targs) args @@ fun h tree result =>
+      verify_place_expr trace h env tree (destination call) @@ fun h tree place ty =>
+      store_to_place trace h env tree place ty result @@ fun h env tree =>
+      match target call with
+        None => Error trace "verify_terminator: Call: target expected" tt
+      | Some bb => Qbb h env tree bb
+      end
   | _ => Error trace "verify_terminator: unsupported terminator" terminator
   end.
 
@@ -620,30 +663,46 @@ Fixpoint verify_basic_blocks
 
 End LocalDecls.
 
-Definition body_is_correct(trace: Trace)(body: Body)(spec: Spec)(tree: SymexTree): Prop :=
+Definition verify_body(trace: Trace)(h: Heap)(tree: SymexTree)(body: Body)(args: list Value)(Q: Heap -> SymexTree -> Value -> Prop): Prop :=
   match local_decls body with
     [] => Error trace "body_is_correct: body has no return local" tt
-  | (result_var_decl::local_decls) as all_local_decls =>
-    let '(params, (local_decls, _)) := combine_ local_decls (inputs body) in
-    let param_tys := map (fun '((name, _), ty) => (name, ty)) params in
-    havoc_vars trace param_tys [] @@ fun env =>
-    produce trace [] env tree (pre spec) @@ fun h env tree =>
-    let env_after_pre := env in
-    process_param_addr_taken_steps trace h env tree @@ fun h env tree =>
-    process_local_addr_taken_steps trace h env tree (result_var_decl::local_decls) @@ fun h env tree cleanup_heapy_locals =>
+  | (result_var_decl::local_decls') =>
+    let '(param_env, (local_decls'', _)) := combine_ local_decls' args in
+    alloc_params trace h tree param_env @@ fun h env tree dealloc_params =>
+    alloc_locals trace h env tree (result_var_decl::local_decls'') @@ fun h env tree dealloc_locals =>
     match basic_blocks body with
       (_, bb)::_ =>
-      verify_basic_blocks all_local_decls trace (basic_blocks body) (List.length (basic_blocks body)) h env tree bb @@ fun h env tree =>
-      cleanup_heapy_locals h tree @@ fun h tree =>
-      match assoc (fst result_var_decl) env with
-        Some (LSValue result) =>
-        consume trace h (("result", LSValue result)::env_after_pre) tree (post spec) @@ fun h env tree =>
-        True
-      | _ => Error trace "body_is_correct: could not find return local in env" (fst result_var_decl, env)
-      end
+      verify_basic_blocks (local_decls body) trace (basic_blocks body) (List.length (basic_blocks body)) h env tree bb @@ fun h env tree =>
+      verify_operand (local_decls body) trace h env tree (Move (fst result_var_decl, [])) @@ fun h tree result _ =>
+      dealloc_locals trace h env tree @@ fun h env tree =>
+      dealloc_params trace h env tree @@ fun h tree =>
+      Q h tree result
     | _ => Error trace "body_is_correct: body has no basic blocks" tt
     end
   end.
+
+Fixpoint forall_tys(trace: Trace)(tys: list Ty)(Q: list Value -> Prop): Prop :=
+  match tys with
+    [] => Q []
+  | ty::tys =>
+    forall_ty trace ty @@ fun v =>
+    forall_tys trace tys @@ fun vs =>
+    Q (v::vs)
+  end.
+
+Definition body_is_correct(trace: Trace)(body: Body)(spec: Spec)(tree: SymexTree): Prop :=
+  if list_eq_dec Ty_eq_dec (map snd (spec_params spec)) (inputs body) then
+    if Ty_eq_dec (spec_output spec) (output body) then
+      forall_tys trace (map snd (spec_params spec)) @@ fun args =>
+      let env := combine (map fst (spec_params spec)) (map (fun v => LSValue (Some v)) args) in
+      produce trace [] env tree (pre spec) @@ fun h env tree =>
+      verify_body trace h tree body args @@ fun h tree result =>
+      consume trace h (("result", LSValue (Some result))::env) tree (post spec) @@ fun h env tree =>
+      True
+    else
+      Error trace "body_is_correct: spec return type does not match body return type" (spec_output spec, output body)
+  else
+    Error trace "body_is_correct: spec parameter type list does not match body parameter type list" (spec_params spec, inputs body).
 
 Definition named_body_is_correct(func_name: string)(body: Body): Prop :=
   let trace := [VerifyingBody func_name] in
