bin/rust/rocq/AxSem.v
@@ -1,0 +1,341 @@
+From iris.base_logic Require Export iprop.
+Require Export VfMir Values.
+
+Parameter value_has_ty0: Ty → Value → Prop.
+
+Inductive value_is_Bool: Value → Prop :=
+  value_is_Bool_intro(b: bool): value_is_Bool (VBool b).
+
+Inductive value_is_RawPtr: Value → Prop :=
+  value_is_RawPtr_intro(ptr: Ptr): value_is_RawPtr (VPtr ptr).
+
+Definition value_has_ty(ty: Ty): Value → Prop :=
+  match ty with
+    Bool => value_is_Bool
+  | RawPtr _ => value_is_RawPtr
+  | _ => value_has_ty0 ty
+  end.
+
+Fixpoint values_have_tys(tys: list Ty)(values: list Value): Prop :=
+  match tys, values with
+    [], [] => True
+  | ty::tys, value::values =>
+    value_has_ty ty value ∧ values_have_tys tys values
+  | _, _ => False
+  end.
+
+Definition Program := list (string * Body).
+Definition Env := string → Ty * Ptr.
+
+Section gfunctors.
+
+Context {Σ: gFunctors}.
+
+Definition points_to(ty: Ty)(ptr: Value)(rhs: Value): iProp Σ.
+Admitted.
+
+Definition points_to_(ty: Ty)(ptr: Value)(rhs: Value): iProp Σ.
+Admitted.
+
+Lemma points_to_def(ty: Ty)(ptr: Value)(rhs: Value):
+  points_to_ ty ptr (VSome rhs) ∗-∗ points_to ty ptr rhs.
+Admitted.
+
+(* [points_to_ ty ptr val] does *NOT* imply [∃ p, ptr = VPtr p]! *)
+Lemma points_to__Tuple0(ptr: Value):
+  ⊢ ∃ v0, points_to_ Tuple0 ptr v0.
+Admitted.
+
+Definition wp_PlaceExprElem(ptr: Value)(ty: Ty)(place_expr_elem: PlaceExprElem)(Q: Value -> Ty -> iProp Σ): iProp Σ.
+Admitted.
+
+Lemma wp_Deref_intro ptr ty ptr' (Q: Value -> Ty -> iProp Σ):
+  points_to ty ptr ptr' ∗ (points_to ty ptr ptr' -∗ ∃ pointee_ty, ⌜ ty = RawPtr pointee_ty ⌝ ∗ Q ptr' pointee_ty) -∗
+  wp_PlaceExprElem ptr ty Deref Q.
+Admitted.
+
+Fixpoint wp_PlaceExprElems ptr ty place_expr_elems Q :=
+  match place_expr_elems with
+    [] => Q ptr ty
+  | place_expr_elem::place_expr_elems =>
+    wp_PlaceExprElem ptr ty place_expr_elem (fun ptr ty =>
+      wp_PlaceExprElems ptr ty place_expr_elems Q)
+  end.
+
+Definition wp_PlaceExpr(env: Env)(place_expr: PlaceExpr)(Q: Value -> Ty -> iProp Σ): iProp Σ :=
+  let '(x, place_expr_elems) := place_expr in
+  let '(ty, ptr) := env x in
+  wp_PlaceExprElems (VPtr ptr) ty place_expr_elems Q.
+
+Definition wp_Operand(env: Env)(operand: Operand)(Q: Value -> Ty -> iProp Σ): iProp Σ.
+Admitted.
+
+Lemma wp_Move_intro(env: Env)(place_expr: PlaceExpr)(Q: Value -> Ty -> iProp Σ):
+  wp_PlaceExpr env place_expr (fun ptr ty =>
+    ∃ v, points_to ty ptr v ∗ (points_to ty ptr v -∗ Q v ty))
+  -∗ wp_Operand env (Move place_expr) Q.
+Admitted.
+
+Lemma wp_Copy_intro(env: Env)(place_expr: PlaceExpr)(Q: Value -> Ty -> iProp Σ):
+  wp_PlaceExpr env place_expr (fun ptr ty =>
+    ∃ v, points_to ty ptr v ∗ (points_to ty ptr v -∗ Q v ty))
+  -∗ wp_Operand env (Copy place_expr) Q.
+Admitted.
+
+Lemma wp_Constant_Tuple0_intro(env: Env)(Q: Value -> Ty -> iProp Σ):
+  Q VTuple0 Tuple0 -∗ wp_Operand env (Constant (Val ZeroSized Tuple0)) Q.
+Admitted.
+
+Definition wp_Rvalue(env: Env)(rvalue: Rvalue)(Q: Value -> Ty -> iProp Σ): iProp Σ.
+Admitted.
+
+Lemma wp_Use_intro(env: Env)(operand: Operand)(Q: Value -> Ty -> iProp Σ):
+  wp_Operand env operand Q -∗ wp_Rvalue env (Use operand) Q.
+Admitted.
+
+Lemma wp_RawPtr__intro(env: Env)(place_expr: PlaceExpr)(Q: Value -> Ty -> iProp Σ):
+  wp_PlaceExpr env place_expr (λ ptr ty, Q ptr (RawPtr ty))
+  -∗ wp_Rvalue env (RawPtr_ place_expr) Q.
+Admitted.
+
+Lemma wp_Cast_PtrToPtr_intro(env: Env)(operand: Operand)(ty: Ty)(Q: Value -> Ty -> iProp Σ):
+  wp_Operand env operand (fun v _ => Q v ty) -∗ wp_Rvalue env (Cast PtrToPtr operand ty) Q. (* We don't support wide pointers yet. *)
+Admitted.
+
+Definition wp_Statement(env: Env)(statement: Statement)(Q: iProp Σ): iProp Σ.
+Admitted.
+
+Lemma wp_Assign_intro(env: Env)(lhs: PlaceExpr)(rhs: Rvalue)(Q: iProp Σ):
+  wp_Rvalue env rhs (fun v ty =>
+    wp_PlaceExpr env lhs (fun ptr ty' =>
+      (∃ state0, points_to_ ty' ptr state0) ∗ (points_to ty' ptr v -∗ Q)))
+  -∗ wp_Statement env (Assign lhs rhs) Q.
+Admitted.
+
+Lemma wp_StorageLive_intro_UNSOUND(env: Env)(x: Local)(Q: iProp Σ): (* SOUNDNESS BUG: Ignored for now. https://github.com/verifast/verifast/issues/948 *)
+  Q -∗ wp_Statement env (StorageLive x) Q.
+Admitted.
+
+Lemma wp_StorageDead_intro_UNSOUND(env: Env)(x: Local)(Q: iProp Σ): (* SOUNDNESS BUG: Ignored for now. https://github.com/verifast/verifast/issues/948 *)
+  Q -∗ wp_Statement env (StorageDead x) Q.
+Admitted.
+
+Lemma wp_Nop_intro(env: Env)(Q: iProp Σ):
+  Q -∗ wp_Statement env Nop Q.
+Admitted.
+
+Fixpoint wp_Statements(env: Env)(statements: list Statement)(Q: iProp Σ): iProp Σ :=
+  match statements with
+    [] => Q
+  | statement::statements =>
+    wp_Statement env statement (wp_Statements env statements Q)
+  end.
+
+Definition BasicBlocks := gmap string BasicBlockData.
+
+Definition wp_Terminator
+    (env: Env)(terminator: Terminator)
+    (wp_call: string -> list GenericArg -> list Value -> (Value -> iProp Σ) -> iProp Σ)
+    (Qbasic_block: BasicBlock -> iProp Σ)
+    (Qreturn: iProp Σ)
+    : iProp Σ.
+Admitted.
+
+Lemma wp_Goto_intro
+    (env: Env)(bb: BasicBlock)
+    (wp_call: string -> list GenericArg -> list Value -> (Value -> iProp Σ) -> iProp Σ)
+    (Qbasic_block: BasicBlock -> iProp Σ)
+    (Qreturn: iProp Σ):
+  ▷ Qbasic_block bb -∗ wp_Terminator env (Goto bb) wp_call Qbasic_block Qreturn.
+Admitted.
+
+Definition wp_SwitchInt
+    (discr: Value)(ty: Ty)(values: list N)(targets: list BasicBlock)
+    (Qbasic_block: BasicBlock -> iProp Σ)
+    : iProp Σ.
+Admitted.
+
+Parameter value_eqb_N: forall (ty: Ty)(value: Value)(n: N), option bool.
+
+Axiom value_eqb_N_Bool_0_eq_true: forall v, value_eqb_N Bool v 0 = Some true → v ≠ VBool true.
+Axiom value_eqb_N_Bool_1_eq_true: forall v, value_eqb_N Bool v 1 = Some true → v = VBool true.
+
+Axiom value_eqb_N_Bool_0_eq_false: forall v, value_eqb_N Bool v 0 = Some false → v = VBool true.
+Axiom value_eqb_N_Bool_1_eq_false: forall v, value_eqb_N Bool v 1 = Some false → v ≠ VBool true.
+
+Lemma wp_SwitchInt_compare
+    (discr: Value)(ty: Ty)(value: N)(values: list N)(target: BasicBlock)(targets: list BasicBlock)
+    (Qbasic_block: BasicBlock → iProp Σ):
+  match value_eqb_N ty discr value with
+    None => True
+  | Some true =>
+    ▷ Qbasic_block target
+  | Some false =>
+    wp_SwitchInt discr ty values targets Qbasic_block
+  end -∗
+  wp_SwitchInt discr ty (value::values) (target::targets) Qbasic_block.
+Admitted.
+
+Lemma wp_SwitchInt_default
+    (discr: Value)(ty: Ty)(target: BasicBlock)
+    (Qbasic_block: BasicBlock → iProp Σ):
+  ▷ Qbasic_block target
+  -∗ wp_SwitchInt discr ty [] [target] Qbasic_block.
+Admitted.
+
+Lemma wp_SwitchInt_intro
+    (env: Env)(discr: Operand)(values: list N)(targets: list BasicBlock)
+    (wp_call: string -> list GenericArg -> list Value -> (Value -> iProp Σ) -> iProp Σ)
+    (Qbasic_block: BasicBlock -> iProp Σ)
+    (Qreturn: iProp Σ):
+  wp_Operand env discr (fun discr ty => wp_SwitchInt discr ty values targets Qbasic_block) -∗
+  wp_Terminator env (SwitchInt discr values targets) wp_call Qbasic_block Qreturn.
+Admitted.
+
+Lemma wp_Return_intro
+    (env: Env)
+    (wp_call: string -> list GenericArg -> list Value -> (Value -> iProp Σ) -> iProp Σ)
+    (Qbasic_block: BasicBlock -> iProp Σ)
+    (Qreturn: iProp Σ):
+  Qreturn -∗ wp_Terminator env Return wp_call Qbasic_block Qreturn.
+Admitted.
+
+Fixpoint wp_Operands(env: Env)(operands: list Operand)(Q: list Value -> iProp Σ): iProp Σ :=
+  match operands with
+    [] => Q []
+  | operand::operands =>
+    wp_Operand env operand (fun v ty =>
+      wp_Operands env operands (fun vs =>
+        Q (v::vs)))
+  end.
+
+Lemma wp_ghost_command_intro env targs args destination target wp_call Qbasic_block Qreturn:
+  ▷ Qbasic_block target -∗
+  wp_Terminator env (Call {|
+    func := Constant (Val ZeroSized (FnDef "VeriFast_ghost_command" targs));
+    args := args;
+    destination := destination;
+    target := Some target
+  |}) wp_call Qbasic_block Qreturn.
+Admitted.
+
+Lemma wp_Call_intro
+    (env: Env)
+    (func_name: string)(targs: GenericArgList)
+    (args: list Operand)(destination: PlaceExpr)(target: option BasicBlock)
+    (wp_call: string -> list GenericArg -> list Value -> (Value -> iProp Σ) -> iProp Σ)
+    (Qbasic_block: BasicBlock -> iProp Σ)
+    (Qreturn: iProp Σ):
+  wp_Operands env args (fun args =>
+    ▷ wp_call func_name (list_of_GenericArgList targs) args (fun result =>
+      wp_PlaceExpr env destination (fun ptr ty =>
+        ∃ state0, points_to_ ty ptr state0 ∗ (points_to ty ptr result -∗
+          match target with
+            None => ⌜ False ⌝
+          | Some basic_block => ▷ Qbasic_block basic_block
+          end))))
+  -∗ wp_Terminator env (Call {|
+       func := Constant (Val ZeroSized (FnDef func_name targs));
+       args := args; destination := destination; target := target
+     |}) wp_call Qbasic_block Qreturn.
+Admitted.
+
+Definition wp_BasicBlock
+    (env: Env)(basic_block: BasicBlockData)
+    (wp_call: string -> list GenericArg -> list Value -> (Value -> iProp Σ) -> iProp Σ)
+    (Qbasic_block: BasicBlock -> iProp Σ)
+    (Qreturn: iProp Σ): iProp Σ :=
+  wp_Statements env (statements basic_block)
+    (wp_Terminator env (terminator basic_block) wp_call Qbasic_block Qreturn).
+
+Definition wp_BasicBlocks
+    (env: Env)(basic_blocks: list (BasicBlock * BasicBlockData))(basic_block_data: BasicBlockData)
+    (wp_call: string -> list GenericArg -> list Value -> (Value -> iProp Σ) -> iProp Σ)
+    (Qreturn: iProp Σ): iProp Σ.
+Admitted. (* To be defined by guarded recursion; involves proving that wp_BasicBlock is contractive in Qbasic_block. *)
+
+Lemma wp_BasicBlocks_intro
+    (env: Env)(basic_blocks: list (BasicBlock * BasicBlockData))(basic_block_data: BasicBlockData)
+    (wp_call: string -> list GenericArg -> list Value -> (Value -> iProp Σ) -> iProp Σ)
+    (Qreturn: iProp Σ):
+  wp_BasicBlock env basic_block_data wp_call (λ bb,
+    match assoc bb basic_blocks with
+      None => False
+    | Some basic_block_data =>
+      wp_BasicBlocks env basic_blocks basic_block_data wp_call Qreturn
+    end) Qreturn
+  -∗ wp_BasicBlocks env basic_blocks basic_block_data wp_call Qreturn.
+Admitted.
+
+Definition wp_Body
+    (body: Body)(args: list Value)
+    (wp_call: string -> list GenericArg -> list Value -> (Value -> iProp Σ) -> iProp Σ)
+    (Q: Value -> iProp Σ)
+    : iProp Σ :=
+  ∀ (env: Env),
+  ⌜ ∀ x info, assoc x (local_decls body) = Some info → ty info = (env x).1 ⌝ -∗
+  ⌜ ∀ x, (env x).2 ≠ null_ptr ⌝ -∗
+  ⌜ Forall (λ '(x, info), assoc x (local_decls body) = Some info) (local_decls body) ⌝ -∗ (* Local variable names are unique *)
+  match local_decls body with
+    [] => False
+  | result_var_decl::local_decls' =>
+    let '(param_env, (local_decls'', _)) := combine_ local_decls' args in
+    ([∗ list] '((x, {| ty := ty |}), v) ∈ param_env, points_to ty (VPtr (snd (env x))) v) -∗
+    ([∗ list] '(x, {| ty := ty |}) ∈ result_var_decl::local_decls'', ∃ state0, points_to_ ty (VPtr (snd (env x))) state0) -∗
+    match basic_blocks body with
+      (_, bb0)::_ =>
+      wp_BasicBlocks env (basic_blocks body) bb0 wp_call
+        (wp_Operand env (Move (fst result_var_decl, [])) (fun result _ =>
+           ([∗ list] '(x, {| ty := ty |}) ∈ result_var_decl::local_decls'', ∃ state, points_to_ ty (VPtr (snd (env x))) state)
+           ∗ ([∗ list] '((x, {| ty := ty |}), _) ∈ param_env, ∃ state, points_to_ ty (VPtr (snd (env x))) state)
+           ∗ Q result))
+    | _ => False
+    end
+  end.
+
+Definition wp_Body'
+    (body: Body)(args: list Value)
+    (wp_call: string -> list GenericArg -> list Value -> (Value -> iProp Σ) -> iProp Σ)
+    (Q: Value -> iProp Σ)
+    : iProp Σ :=
+  ⌜ values_have_tys (inputs body) args ⌝ -∗
+  wp_Body body args wp_call (λ result, (⌜ value_has_ty (output body) result ⌝ -∗ Q result)%I).
+
+Definition wp_call_std
+    (wp_call: string -> list GenericArg -> list Value -> (Value -> iProp Σ) -> iProp Σ)
+    (func_name: string)(targs: list GenericArg)(args: list Value)
+    (Q: Value -> iProp Σ)
+    : iProp Σ :=
+  if string_dec func_name "std::ptr::mut_ptr::<impl *mut T>::is_null" then
+    match args with
+      [ptr] => Q (VBool (value_eqb ptr (VPtr null_ptr)))
+    | _ => False%I
+    end
+  else if string_dec func_name "std::ptr::null_mut" then
+    Q (VPtr null_ptr)
+  else if string_dec func_name "std::process::abort" then
+    True%I
+  else
+    wp_call func_name targs args Q.
+
+Definition wp_Program
+    (program: Program)
+    (func_name: string)(targs: list GenericArg)(args: list Value)(Q: Value -> iProp Σ)
+    : iProp Σ.
+Admitted. (* To be defined using guarded recursion, exploiting the contractiveness of wp_Body in wp_call *)
+
+Lemma wp_Program_intro
+    (program: Program)
+    (func_name: string)(targs: list GenericArg)(args: list Value)(Q: Value -> iProp Σ):
+  match assoc func_name program with
+    None => True (* We ignore non-closed programs *)
+  | Some body =>
+    wp_Body' body args (wp_call_std (wp_Program program)) Q
+  end -∗
+  wp_Program program func_name targs args Q.
+Admitted.
+
+Definition program_has_no_ub(program: Program): Prop :=
+  ⊢ wp_Program program "main" [] [] (fun _ => True).
+
+End gfunctors.
