bin/rust/rocq/SymexSoundness.v
@@ -1,0 +1,1646 @@
+From iris.proofmode Require Import proofmode.
+Require Export AxSem LogicalHeaps.
+
+Section gfunctors.
+
+Context {Σ: gFunctors}.
+
+Parameter lh_big_ast: forall (H: LogHeap) (f: PrimChunk → iProp Σ), iProp Σ.
+Axiom lh_big_ast_lh_comp_intro:
+  forall (H1 H2: LogHeap) (f: PrimChunk → iProp Σ),
+  lh_big_ast H1 f ∗ lh_big_ast H2 f -∗ lh_big_ast (H1 ⋅ H2) f.
+Axiom lh_big_ast_lh_comp_elim:
+  forall (H1 H2: LogHeap) (f: PrimChunk → iProp Σ),
+  lh_big_ast (H1 ⋅ H2) f -∗ lh_big_ast H1 f ∗ lh_big_ast H2 f.
+Axiom lh_big_ast_lh_sing_intro:
+  forall chunk f,
+  f chunk -∗ lh_big_ast {[+ chunk +]} f.
+Axiom lh_big_ast_lh_sing_elim:
+  forall chunk f,
+  lh_big_ast {[+ chunk +]} f -∗ f chunk.
+Axiom lh_big_ast_lh_empty_intro:
+  forall f,
+  ⊢ lh_big_ast ∅ f. 
+
+Definition own_logheap(H: LogHeap): iProp Σ :=
+  lh_big_ast H (λ '(PointsTo_ ty ptr v), points_to_ ty ptr v).
+
+Lemma own_logheap_lh_comp_intro H1 H2:
+  own_logheap H1 ∗ own_logheap H2 -∗ own_logheap (H1 ⋅ H2).
+Proof.
+  apply lh_big_ast_lh_comp_intro.
+Qed.
+
+Lemma own_logheap_lh_comp_elim H1 H2:
+  own_logheap (H1 ⋅ H2) -∗ own_logheap H1 ∗ own_logheap H2.
+Proof.
+  apply lh_big_ast_lh_comp_elim.
+Qed.
+
+Lemma own_logheap_lh_empty_intro:
+  ⊢ own_logheap ∅.
+Proof.
+  unfold own_logheap.
+  iApply lh_big_ast_lh_empty_intro.
+Qed.
+
+Definition place_as_ptr(env: AxSem.Env)(place: Place): Value :=
+  match place with
+    PNonAddrTakenLocal x => VPtr (snd (env x))
+  | PDeref ptr => ptr
+  end.
+
+Section preds.
+
+Variable preds: list (string * PredDef).
+
+Definition own_heap(h: Heap): iProp Σ :=
+  ∃ H,
+  ⌜ heap_holds preds H h ⌝ ∗
+  own_logheap H.
+
+Definition own_chunk(chunk: Chunk): iProp Σ :=
+  ∃ H, ⌜ chunk_holds preds H chunk ⌝ ∗ own_logheap H.
+
+Lemma own_chunk_prim_intro ty ptr v:
+  points_to_ ty ptr v -∗
+  own_chunk (Prim (PointsTo_ ty ptr v)).
+Proof.
+  iIntros "Hptr".
+  unfold own_chunk.
+  iExists {[+ PointsTo_ ty ptr v +]}.
+  iSplitL "". {
+    iPureIntro.
+    constructor.
+  }
+  unfold own_logheap.
+  iApply (lh_big_ast_lh_sing_intro).
+  iAssumption.
+Qed.
+
+Lemma own_heap_cons_intro(chunk: Chunk)(h: Heap):
+  own_chunk chunk -∗
+  own_heap h -∗
+  own_heap (chunk::h).
+Proof.
+  unfold own_chunk, own_heap.
+  iIntros "[%Hchunk [%HHchunk HHchunk]] [%Hh [%HHh HHh]]".
+  iExists (Hchunk ⋅ Hh).
+  iSplitL "". {
+    iPureIntro.
+    simpl.
+    exists Hchunk.
+    exists Hh.
+    split. reflexivity.
+    tauto.
+  }
+  iApply (own_logheap_lh_comp_intro).
+  iFrame.
+Qed.
+
+Definition own_env_entry(Γ: AxSem.Env)(x: string)(state: LocalState): iProp Σ :=
+  match state with
+    LSValue (Some v) => points_to (fst (Γ x)) (VPtr (snd (Γ x))) v
+  | LSValue None => ∃ v, points_to_ (fst (Γ x)) (VPtr (snd (Γ x))) v
+  | LSPlace ptr => ⌜ ptr = snd (Γ x) ⌝
+  end.
+
+Fixpoint own_env(Γ: AxSem.Env)(env: Env): iProp Σ :=
+  match env with
+    [] => True
+  | (x, state)::env => own_env_entry Γ x state ∗ own_env Γ env
+  end.
+
+Inductive place_has_ty(Γ: AxSem.Env): Place -> Ty -> Prop :=
+| PNonAddrTakenLocal_has_ty x:
+  place_has_ty Γ (PNonAddrTakenLocal x) (fst (Γ x))
+| PDeref_has_ty ptr ty:
+  place_has_ty Γ (PDeref ptr) ty
+.
+
+Lemma load_from_non_addr_taken_local Γ env x v:
+  assoc x env = Some (LSValue (Some v)) →
+  own_env Γ env -∗
+  points_to (Γ x).1 (VPtr (Γ x).2) v ∗
+  (points_to (Γ x).1 (VPtr (Γ x).2) v -∗ own_env Γ env).
+Proof.
+  induction env.
+  - (* nil *)
+    intros.
+    discriminate.
+  - (* cons *)
+    destruct a as [x' state].
+    intros.
+    simpl in *.
+    destruct (string_dec x x').
+    + subst.
+      injection H; clear H; intros; subst.
+      iStartProof.
+      iIntros "[H11 H12]".
+      iSplitL "H11".
+      * iExact "H11".
+      * iIntros "H2".
+        iSplitL "H2"; iAssumption.
+    + apply IHenv in H.
+      iStartProof.
+      iIntros "[H1 H2]".
+      iPoseProof (H with "H2") as "[H H']".
+      iSplitL "H".
+      iExact "H".
+      iIntros "H".
+      iSplitL "H1".
+      iAssumption.
+      iApply "H'".
+      iAssumption.
+Qed.
+
+Lemma remove1_assoc_own_env x env v0 env' Γ:
+  remove1_assoc x env = Some (LSValue v0, env') →
+  own_env Γ env -∗
+  (∃ v0, points_to_ (Γ x).1 (VPtr (Γ x).2) v0) ∗
+  own_env Γ env'.
+Proof.
+  revert env'.
+  induction env as [|x'_state env]; simpl; intro env'.
+  - (* nil *)
+    discriminate.
+  - (* cons *)
+    destruct x'_state as [x' state].
+    destruct (string_dec x' x).
+    + (* x' = x *)
+      subst.
+      intros H; injection H; intros; subst.
+      iIntros "[Hx Henv']".
+      iSplitL "Hx". {
+        simpl.
+        destruct v0.
+        - (* Some v *)
+          iExists (VSome v).
+          iApply (points_to_def with "Hx").
+        - (* None *)
+          iAssumption.
+      }
+      iAssumption.
+    + (* x' ≠ x *)
+      destruct (remove1_assoc x env) as [[state0 env'']|].
+      * (* Some *)
+        intro Hstate0.
+        injection Hstate0; intros; subst.
+        iIntros "[Hx' Henv]".
+        simpl.
+        iDestruct ((IHenv env'') with "Henv") as "Henv".
+        reflexivity.
+        iFrame.
+        iFrame.
+      * (* None *)
+        intros; discriminate.
+Qed.
+
+Lemma place_local_ptr_eq Γ env x ptr:
+  assoc x env = Some (LSPlace ptr) →
+  own_env Γ env -∗
+  ⌜ ptr = (Γ x).2 ⌝ ∗
+  own_env Γ env.
+Proof.
+  induction env.
+  - (* nil *)
+    intros.
+    discriminate.
+  - (* cons *)
+    simpl; intros.
+    destruct a as [x0 state].
+    destruct (string_dec x x0).
+    + (* x = x0 *)
+      subst.
+      injection H; intros; subst.
+      iIntros "[Hx0 Henv]".
+      simpl in *.
+      iDestruct "Hx0" as %Hx0.
+      subst.
+      iSplitL "". {
+        iPureIntro.
+        reflexivity.
+      }
+      iSplitL "". {
+        iPureIntro.
+        reflexivity.
+      }
+      iAssumption.
+    + (* x ≠ x0 *)
+      iIntros "[Hx0 Henv]".
+      iDestruct (IHenv H with "Henv") as "Henv".
+      iFrame.
+      iAssumption.
+Qed.
+
+Lemma consume_points_to_sound trace h tree ty ptr Qsymex Q:
+  consume_points_to trace h tree ty ptr Qsymex →
+  (∀ h tree v, ⌜ Qsymex h tree v ⌝ -∗ own_heap h -∗ Q v) -∗
+  own_heap h -∗
+  ∃ v,
+  points_to ty ptr v ∗ Q v.
+Proof.
+  intros Hconsume.
+  unfold own_heap.
+  iIntros "HQ Hh".
+  iDestruct "Hh" as (H) "[Hh HH]".
+  iDestruct "Hh" as %Hh.
+  apply consume_points_to_sound with (1:=Hh) in Hconsume.
+  destruct Hconsume as (H' & h' & tree' & v & HHeq & Hh' & HQsymex).
+  iExists v.
+  subst.
+  unfold own_logheap.
+  iPoseProof (lh_big_ast_lh_comp_elim with "HH") as "HH".
+  iDestruct "HH" as "[Hpoints_to_ HH']".
+  iPoseProof (lh_big_ast_lh_sing_elim with "Hpoints_to_") as "Hpoints_to_".
+  iSplitL "Hpoints_to_". {
+    iApply (points_to_def with "Hpoints_to_").
+  }
+  iApply ("HQ" with "[% //]").
+  iExists H'.
+  iSplitL "". {
+    iPureIntro.
+    assumption.
+  }
+  iAssumption.
+Qed.
+
+Lemma consume_points_to__sound trace h tree ty ptr Qsymex:
+  consume_points_to_ trace h tree ty ptr Qsymex →
+  ∀ Q,
+  (∀ h tree v, ⌜ Qsymex h tree v ⌝ -∗ own_heap h -∗ Q v) -∗
+  own_heap h -∗
+  ∃ v,
+  points_to_ ty ptr v ∗ Q v.
+Proof.
+  intros Hconsume Q.
+  unfold own_heap.
+  iIntros "HQ Hh".
+  iDestruct "Hh" as (H) "[Hh HH]".
+  iDestruct "Hh" as %Hh.
+  apply consume_points_to__sound with (1:=Hh) in Hconsume.
+  destruct Hconsume as (H' & h' & tree' & v & HHeq & Hh' & HQsymex).
+  iExists v.
+  subst.
+  unfold own_logheap.
+  iPoseProof (lh_big_ast_lh_comp_elim with "HH") as "HH".
+  iDestruct "HH" as "[Hpoints_to_ HH']".
+  iPoseProof (lh_big_ast_lh_sing_elim with "Hpoints_to_") as "Hpoints_to_".
+  iFrame.
+  iApply ("HQ" with "[% //]").
+  iExists H'.
+  iSplitL "". {
+    iPureIntro.
+    assumption.
+  }
+  iAssumption.
+Qed.
+
+Lemma load_from_pointer_sound trace h tree ty ptr Qsymex Q:
+  load_from_pointer trace h tree ty ptr Qsymex →
+  (∀ h tree v, ⌜ Qsymex h tree v ⌝ -∗ own_heap h -∗ Q v) -∗
+  own_heap h -∗
+  ∃ v,
+  points_to ty ptr v ∗
+  (points_to ty ptr v -∗ Q v).
+Proof.
+  intros Hload.
+  unfold load_from_pointer in Hload.
+  apply consume_points_to_sound with (Q:=λ v, (points_to ty ptr v -∗ Q v)%I) in Hload.
+  iIntros "HQ Hh".
+  iApply (Hload with "[HQ] Hh").
+  unfold own_heap.
+  iIntros (h0 tree0 v) "%HQsymex Hh0 Hpoints_to". 
+  iDestruct "Hh0" as (H0) "[%Hh0 HH0]".
+  iApply ("HQ" with "[% //]").
+  iExists ({[+ PointsTo_ ty ptr (VSome v) +]} ⋅ H0).
+  iSplitL "". {
+    iPureIntro.
+    simpl.
+    exists {[+ PointsTo_ ty ptr (VSome v) +]}.
+    exists H0.
+    tauto.
+  }
+  unfold own_logheap.
+  iApply lh_big_ast_lh_comp_intro.
+  iSplitL "Hpoints_to". {
+    iApply lh_big_ast_lh_sing_intro.
+    iApply points_to_def.
+    iAssumption.
+  }
+  iAssumption.
+Qed.
+
+Lemma load_from_place_sound trace h env tree place ty Qsymex Γ Q:
+  load_from_place trace h env tree place ty Qsymex →
+  place_has_ty Γ place ty →
+  (∀ h tree v, ⌜ Qsymex h tree v ⌝ -∗ own_heap h -∗ own_env Γ env -∗ Q v) -∗
+  own_heap h -∗
+  own_env Γ env -∗
+  ∃ v,
+  points_to ty (place_as_ptr Γ place) v ∗
+  (points_to ty (place_as_ptr Γ place) v -∗
+   Q v).
+Proof.
+  intros.
+  iStartProof.
+  iIntros "HQ Hh Henv".
+  destruct place.
+  - (* PNonAddrTakenLocal *)
+    simpl in H.
+    simpl.
+    inversion H0; subst.
+    case_eq (assoc x env); intros; rewrite H1 in H; try tauto.
+    rename l into state.
+    destruct state; try tauto.
+    destruct v; try tauto.
+    iExists v.
+    iPoseProof (load_from_non_addr_taken_local with "Henv") as "[H1 H2]".
+    apply H1.
+    iSplitL "H1". iAssumption.
+    iIntros "H".
+    iPoseProof ("HQ" with "[% //] Hh") as "H'".
+    iApply "H'".
+    iApply "H2".
+    iAssumption.
+  - (* PDeref *)
+    simpl in H.
+    apply load_from_pointer_sound with (Q:=Q) in H.
+    iApply (H with "[HQ Henv] Hh").
+    iIntros (h0 tree0 v) "%HQsymex Hh0".
+    iApply ("HQ" with "[% //] Hh0 Henv").
+Qed.
+
+Lemma store_to_place_sound trace h env tree place ty v Qsymex Γ Q:
+  store_to_place trace h env tree place ty v Qsymex →
+  place_has_ty Γ place ty →
+  (∀ h env tree, ⌜ Qsymex h env tree ⌝ -∗ own_heap h -∗ own_env Γ env -∗ Q) -∗
+  own_heap h -∗
+  own_env Γ env -∗
+  (∃ v0, points_to_ ty (place_as_ptr Γ place) v0) ∗
+  (points_to ty (place_as_ptr Γ place) v -∗
+   Q).
+Proof.
+  intros Hstore Hplace_has_ty.
+  iIntros "HQ Hh Henv".
+  unfold store_to_place in Hstore.
+  destruct (Ty_eq_dec ty Tuple0).
+  - (* ty = Tuple0 *)
+    subst.
+    iSplitL "". {
+      iApply points_to__Tuple0.
+    }
+    iIntros.
+    iApply ("HQ" with "[% //] Hh Henv").
+  - destruct place.
+    + (* PNonAddrTakenLocal *)
+      simpl.
+      case_eq (remove1_assoc x env). 2:{
+        intro Hx; rewrite Hx in Hstore; tauto.
+      }
+      intros [y' xys'] Hxys'.
+      rewrite Hxys' in Hstore.
+      destruct y'; try tauto.
+      iDestruct ("HQ" with "[% //] Hh") as "HQ".
+      inversion Hplace_has_ty; subst.
+      iDestruct ((remove1_assoc_own_env _ _ _ _ _ Hxys') with "Henv") as "[Hx Henv]".
+      iFrame.
+      iIntros "Hx".
+      simpl.
+      iApply ("HQ" with "[Hx Henv]").
+      iFrame.
+    + (* PDeref *)
+      simpl in *.
+      eapply consume_points_to__sound with (Q:=λ _, (points_to ty ptr v -∗ Q)%I) in Hstore.
+      iDestruct (Hstore with "[HQ Henv] Hh") as "HQ".
+      * iIntros (h0 tree0 v0) "HQ' Hh0 Hptr".
+        iApply ("HQ" with "HQ' [Hh0 Hptr] Henv").
+        unfold own_heap.
+        iDestruct "Hh0" as (H) "[Hh0 HH]".
+        iDestruct "Hh0" as %Hh0.
+        simpl.
+        iExists ({[+ PointsTo_ ty ptr (VSome v) +]} ⋅ H).
+        iSplitL "". {
+          iPureIntro.
+          exists {[+ PointsTo_ ty ptr (VSome v) +]}.
+          exists H.
+          split. reflexivity.
+          split. reflexivity.
+          assumption.
+        }
+        unfold own_logheap.
+        iApply lh_big_ast_lh_comp_intro.
+        iSplitL "Hptr". {
+          iApply lh_big_ast_lh_sing_intro.
+          iApply points_to_def.
+          iAssumption.
+        }
+        iAssumption.
+      * iDestruct "HQ" as (v0) "[Hptr HQ]".
+        iSplitL "Hptr". {
+          iExists v0.
+          iAssumption.
+        }
+        iAssumption.
+Qed.
+
+Section specs.
+
+Variable specs: list (string * Spec).
+
+Section Γ.
+
+Variable Γ: AxSem.Env.
+
+Hypothesis Γ_non_null: ∀ x, (Γ x).2 ≠ null_ptr.
+
+Section local_decls.
+
+Variable local_decls: list (Local * LocalDecl).
+
+Hypothesis Γ_well_typed: ∀ x local_decl,
+  assoc x local_decls = Some local_decl → ty local_decl = (Γ x).1.
+
+Lemma verify_local_sound trace env x Qsymex ty vptr Q:
+  verify_local local_decls trace env x Qsymex →
+  vptr = VPtr (Γ x).2 →
+  ty = (Γ x).1 →
+  (∀ place,
+   ⌜ Qsymex place ty ⌝ -∗
+   ⌜ place_has_ty Γ place ty ⌝ -∗
+   own_env Γ env -∗
+   Q (place_as_ptr Γ place) ty) -∗
+  own_env Γ env -∗
+  Q vptr ty.
+Proof.
+  unfold verify_local.
+  case_eq (assoc x local_decls); intros; try tauto.
+  pose proof (Γ_well_typed _ _ H).
+  subst.
+  destruct l.
+  simpl in H3.
+  subst.
+  case_eq (assoc x env); intros; rewrite H1 in H0; try tauto.
+  iIntros  "HQ Henv".
+  destruct l.
+  * iApply ("HQ" with "[% //] [%] Henv").
+    apply PNonAddrTakenLocal_has_ty.
+  * iDestruct (place_local_ptr_eq with "Henv") as "[%Ha Henv]". {
+      eassumption.
+    }
+    subst.
+    iApply ("HQ" with "[% //] [%] Henv").
+    constructor.
+Qed.
+
+Lemma verify_place_expr_elem_sound trace h env tree place ty place_expr_elem Qsymex ptr Q:
+  verify_place_expr_elem trace h env tree place ty place_expr_elem Qsymex →
+  place_has_ty Γ place ty →
+  ptr = place_as_ptr Γ place →
+  (∀ h tree place ty,
+   ⌜ Qsymex h tree place ty ⌝ -∗
+   ⌜ place_has_ty Γ place ty ⌝ -∗
+   own_heap h -∗ own_env Γ env -∗ Q (place_as_ptr Γ place) ty) -∗
+  own_heap h -∗
+  own_env Γ env -∗
+  wp_PlaceExprElem ptr ty place_expr_elem Q.
+Proof.
+  intros Hverify Hty Hptr.
+  iIntros "HQ".
+  subst.
+  destruct place_expr_elem.
+  - (* Deref *)
+    unfold verify_place_expr_elem in Hverify.
+    iIntros "Hh Henv".
+    eapply load_from_place_sound with (2:=Hty) in Hverify.
+    iDestruct (Hverify with "[HQ] Hh Henv") as "Hverify". 2: {
+      iDestruct "Hverify" as (v) "[Hpoints_to HQ']".
+      iApply wp_Deref_intro.
+      iFrame.
+    }
+    iIntros (h0 tree0 v) "%HQ Hh0 Henv".
+    destruct ty; try tauto.
+    iExists ty.
+    iSplitL "". {
+      iPureIntro.
+      reflexivity.
+    }
+    iApply ("HQ" with "[% //] [%] Hh0 Henv").
+    constructor.
+Qed.
+
+Lemma verify_place_expr_elems_sound trace h env tree place ty place_expr_elems Qsymex ptr Q:
+  verify_place_expr_elems trace h env tree place ty place_expr_elems Qsymex →
+  place_has_ty Γ place ty →
+  ptr = place_as_ptr Γ place →
+  (∀ h tree place ty,
+   ⌜ Qsymex h tree place ty ⌝ -∗
+   ⌜ place_has_ty Γ place ty ⌝ -∗
+   own_heap h -∗ own_env Γ env -∗ Q (place_as_ptr Γ place) ty) -∗
+  own_heap h -∗
+  own_env Γ env -∗
+  wp_PlaceExprElems ptr ty place_expr_elems Q.
+Proof.
+  revert trace h env tree place ty Qsymex ptr Q.
+  induction place_expr_elems.
+  - (* nil *)
+    intros.
+    simpl in *.
+    subst.
+    iIntros "HQ".
+    iApply ("HQ" with "[% //] [% //]").
+  - (* cons *)
+    intros. iIntros "HQ Hh Henv".
+    simpl in *.
+    eapply verify_place_expr_elem_sound in H; try eassumption.
+    iApply (H with "[HQ] Hh Henv").
+    iIntros (h0 tree0 place0 ty0) "%Hverify %Hplace0 Hh0 Henv".
+    eapply IHplace_expr_elems in Hverify; try assumption.
+    iApply (Hverify with "HQ Hh0 Henv").
+    reflexivity.
+Qed.
+
+Lemma verify_place_expr_sound trace h env tree place_expr Qsymex Q:
+  verify_place_expr local_decls trace h env tree place_expr Qsymex →
+  (∀ h tree place ty,
+   ⌜ Qsymex h tree place ty ⌝ -∗
+   ⌜ place_has_ty Γ place ty ⌝ -∗
+   own_heap h -∗ own_env Γ env -∗ Q (place_as_ptr Γ place) ty) -∗
+  own_heap h -∗
+  own_env Γ env -∗
+  wp_PlaceExpr Γ place_expr Q.
+Proof.
+  intros Hverify. iIntros "HQ".
+  destruct place_expr as [x place_expr_elems].
+  simpl in *.
+  case_eq (Γ x); intros ty ptr Hx.
+  iIntros "Hh Henv".
+  iRevert "Henv Hh".
+  iApply ((verify_local_sound _ _ _ _ _ (VPtr ptr) (λ vptr ty, (own_heap h -∗ wp_PlaceExprElems vptr ty place_expr_elems Q)%I))).
+  - apply Hverify.
+  - rewrite Hx; reflexivity.
+  - rewrite Hx; reflexivity.
+  - iIntros (place) "%Hverify' %Hplace Henv Hh".
+    iRevert "Hh Henv".
+    iApply verify_place_expr_elems_sound.
+    + apply Hverify'.
+    + assumption.
+    + reflexivity.
+    + iAssumption.
+Qed.
+
+Lemma verify_operand_sound trace h env tree operand Qsymex Q:
+  verify_operand local_decls trace h env tree operand Qsymex →
+  (∀ h tree v ty,
+   ⌜ Qsymex h tree v ty ⌝ -∗
+   own_heap h -∗ own_env Γ env -∗ Q v ty) -∗
+  own_heap h -∗ own_env Γ env -∗ wp_Operand Γ operand Q.
+Proof.
+  destruct operand; simpl; intros Hverify; iIntros "HQ Hh Henv".
+  - (* Move *)
+    iApply wp_Move_intro.
+    iRevert "Hh Henv".
+    iApply verify_place_expr_sound; try eassumption.
+    iIntros (h0 tree0 place0 ty) "%Hload %Hplace_has_ty".
+    iApply load_from_place_sound; try eassumption.
+    iIntros (h1 tree1 v) "%HQ'".
+    iDestruct ("HQ" with "[% //]") as "HQ".
+    iAssumption.
+  - (* Copy *)
+    iApply wp_Copy_intro.
+    iRevert "Hh Henv".
+    iApply verify_place_expr_sound; try eassumption.
+    iIntros (h0 tree0 place0 ty) "%Hload %Hplace_has_ty".
+    iApply load_from_place_sound; try eassumption.
+    iIntros (h1 tree1 v) "%HQ'".
+    iApply ("HQ" with "[% //]").
+  - (* Constant *)
+    destruct const; try tauto.
+    destruct value; try tauto.
+    destruct ty; try tauto.
+    iApply wp_Constant_Tuple0_intro.
+    iApply ("HQ" with "[% //] Hh Henv").
+Qed.
+
+Lemma verify_operands_sound trace h env tree operands Qsymex Q:
+  verify_operands local_decls trace h env tree operands Qsymex →
+  (∀ h tree vs,
+   ⌜ Qsymex h tree vs ⌝ -∗
+   own_heap h -∗ own_env Γ env -∗ Q vs) -∗
+  own_heap h -∗ own_env Γ env -∗ wp_Operands Γ operands Q.
+Proof.
+  revert trace h env tree Qsymex Q.
+  induction operands as [|operand operands]; simpl.
+  - (* nil *)
+    iIntros (trace h env tree Qsymex Q Hverify) "HQ Hh Henv".
+    iApply ("HQ" with "[% //] Hh Henv").
+  - (* cons *)
+    iIntros (trace h env tree Qsymex Q Hverify) "HQ Hh Henv".
+    iApply (verify_operand_sound with "[HQ] Hh Henv"); try eassumption.
+    clear Hverify.
+    iIntros (h0 tree0 v ty) "%Hverify Hh0 Henv".
+    iApply (IHoperands with "[HQ] Hh0 Henv"); try eassumption.
+    clear Hverify.
+    iIntros (h1 tree1 vs) "%Hverify Hh1 Henv".
+    iApply ("HQ" with "[% //] Hh1 Henv").
+Qed.
+
+Lemma verify_rvalue_sound trace h env tree rvalue Qsymex Q:
+  verify_rvalue local_decls trace h env tree rvalue Qsymex →
+  (∀ h tree v ty,
+   ⌜ Qsymex h tree v ty ⌝ -∗
+   own_heap h -∗ own_env Γ env -∗ Q v ty) -∗
+  own_heap h -∗ own_env Γ env -∗ wp_Rvalue Γ rvalue Q.
+Proof.
+  destruct rvalue; simpl; intros Hverify; iIntros "HQ Hh Henv".
+  - (* Use *)
+    iApply wp_Use_intro.
+    iRevert "Hh Henv".
+    iApply verify_operand_sound; try eassumption.
+    iApply "HQ".
+  - (* RawPtr_ *)
+    iApply wp_RawPtr__intro.
+    iRevert "Hh Henv".
+    iApply verify_place_expr_sound; try eassumption.
+    iIntros (h0 tree0 place0 ty) "%HQ' %Hplace".
+    destruct place0; try tauto.
+    iApply ("HQ" with "[% //]").
+  - (* Cast *)
+    destruct kind; try tauto.
+    iApply wp_Cast_PtrToPtr_intro.
+    iRevert "Hh Henv".
+    iApply verify_operand_sound; try eassumption.
+    iIntros (h0 tree0 v ty') "%HQ'".
+    iApply ("HQ" with "[% //]").
+Qed.
+
+(* TODO: Once we support StorageLive and StorageDead, Γ will not be fixed across statement execution. *)
+
+Lemma verify_statement_sound trace h env tree statement Qsymex Q:
+  verify_statement local_decls trace h env tree statement Qsymex →
+  (∀ h env tree,
+   ⌜ Qsymex h env tree ⌝ -∗ own_heap h -∗ own_env Γ env -∗ Q) -∗
+  own_heap h -∗ own_env Γ env -∗ wp_Statement Γ statement Q.
+Proof.
+  destruct statement; simpl; intros Hverify; iIntros "HQ Hh Henv".
+  - (* Assign *)
+    iApply wp_Assign_intro.
+    iRevert "Hh Henv".
+    iApply verify_rvalue_sound; try eassumption.
+    iIntros (h0 tree0 v ty) "%Hverify'".
+    iApply verify_place_expr_sound; try eassumption.
+    iIntros (h1 tree1 place ty0) "%Hstore %Hplace_has_ty".
+    iApply store_to_place_sound; try eassumption.
+    iAssumption.
+  - (* StorageLive *)
+    iApply wp_StorageLive_intro_UNSOUND.
+    iApply ("HQ" with "[% //] Hh Henv").
+  - (* StorageDead *)
+    iApply wp_StorageDead_intro_UNSOUND.
+    iApply ("HQ" with "[% //] Hh Henv").
+  - (* Nop *)
+    iApply wp_Nop_intro.
+    iApply ("HQ" with "[% //] Hh Henv").
+Qed.
+
+Lemma verify_statements_sound trace h env tree statements Qsymex Q:
+  verify_statements local_decls trace h env tree statements Qsymex →
+  (∀ h env tree,
+   ⌜ Qsymex h env tree ⌝ → own_heap h -∗ own_env Γ env -∗ Q) -∗
+  own_heap h -∗ own_env Γ env -∗ wp_Statements Γ statements Q.
+Proof.
+  revert trace h env tree Qsymex Q.
+  induction statements.
+  - (* nil *)
+    intros trace h env tree Qsymex Q Hverify; iIntros "HQ".
+    iApply ("HQ" with "[% //]").
+  - (* cons *)
+    intros trace h env tree Qsymex Q Hverify; iIntros "HQ".
+    simpl in *.
+    iApply verify_statement_sound; try eassumption.
+    iIntros (h0 env0 tree0) "%Hverify_statements".
+    iApply IHstatements; try eassumption.
+    iAssumption.
+Qed.
+
+Lemma assume_value_eq_N_sound trace v ty value Q:
+  assume_value_eq_N trace v ty value Q →
+  value_eqb_N ty v value = Some true →
+  Q.
+Proof.
+  intros Hassume Heq.
+  destruct value as [|[ | | ]]; destruct ty; simpl in Hassume; try tauto.
+  - (* 0%N *)
+    apply value_eqb_N_Bool_0_eq_true in Heq.
+    tauto.
+  - (* 1%N *)
+    apply value_eqb_N_Bool_1_eq_true in Heq.
+    tauto.
+Qed.
+
+Lemma assume_value_neq_N_sound trace v ty value Q:
+  assume_value_neq_N trace v ty value Q →
+  value_eqb_N ty v value = Some false →
+  Q.
+Proof.
+  intros Hassume Hneq.
+  destruct value as [|[ | | ]]; destruct ty; simpl in Hassume; try tauto.
+  - (* 0%N *)
+    apply value_eqb_N_Bool_0_eq_false in Hneq.
+    tauto.
+  - (* 1%N *)
+    apply value_eqb_N_Bool_1_eq_false in Hneq.
+    tauto.
+Qed.
+
+Lemma verify_switch_int_sound trace tree discr ty values targets Qsymex_bb (Qbb: BasicBlock → iProp Σ):
+  verify_switch_int trace tree discr ty values targets Qsymex_bb →
+  ▷ (∀ tree bb, ⌜ Qsymex_bb tree bb ⌝ -∗ Qbb bb) -∗
+  wp_SwitchInt discr ty values targets Qbb.
+Proof.
+  revert trace tree targets.
+  induction values as [|value values]; intros trace tree targets Hverify; iIntros "HQ".
+  - (* nil *)
+    destruct targets as [|target [|?]]; simpl in Hverify; try tauto.
+    iApply wp_SwitchInt_default.
+    iNext.
+    iApply "HQ".
+    iPureIntro.
+    apply Hverify.
+  - (* cons *)
+    destruct targets as [|target targets]; try tauto.
+    destruct tree; try tauto.
+    simpl in Hverify.
+    destruct Hverify as [Hverify_neq Hverify_eq].
+    iApply wp_SwitchInt_compare.
+    case_eq (value_eqb_N ty discr value).
+    + (* Some *)
+      intros b Hb.
+      destruct b.
+      * (* true *)
+        apply assume_value_eq_N_sound with (2:=Hb) in Hverify_eq.
+        iNext.
+        iApply "HQ".
+        iPureIntro.
+        apply Hverify_eq.
+      * (* false *)
+        apply assume_value_neq_N_sound with (2:=Hb) in Hverify_neq.
+        iApply IHvalues.
+        apply Hverify_neq.
+        iNext.
+        iAssumption.
+    + (* None *)
+      intros.
+      iPureIntro.
+      constructor.
+Qed.
+
+Definition own_asn(env: Env)(a: Asn)(env': Env): iProp Σ :=
+  ∃ H: LogHeap, ⌜ asn_holds preds H env a env' ⌝ ∗ own_logheap H.
+
+Lemma produce_sound trace h env tree a Qsymex env' Q:
+  produce trace h env tree a Qsymex →
+  (∀ h tree,
+   ⌜ Qsymex h env' tree ⌝ -∗
+   own_heap h -∗ Q) -∗
+  own_heap h -∗
+  own_asn env a env' -∗
+  Q.
+Proof.
+  intros Hproduce.
+  iIntros "HQ Hh Ha".
+  unfold own_heap.
+  unfold own_asn.
+  iDestruct "Hh" as (H) "[%Hh HH]".
+  iDestruct "Ha" as (H0) "[%Ha HH0]".
+  apply produce_sound with (1:=Hh) (2:=Ha) in Hproduce.
+  destruct Hproduce as (h' & tree' & HQsymex & Hh').
+  iApply ("HQ" with "[% //]").
+  iExists (H ⋅ H0).
+  iSplitL "". {
+    iPureIntro.
+    assumption.
+  }
+  iApply own_logheap_lh_comp_intro.
+  iFrame.
+Qed.
+
+Lemma consume_sound trace h env tree a Qsymex Q:
+  consume trace h env tree a Qsymex →
+  (∀ h env' tree,
+   ⌜ Qsymex h env' tree ⌝ -∗
+   own_asn env a env' ∗ own_heap h -∗ Q) -∗
+  own_heap h -∗
+  Q.
+Proof.
+  intros Hconsume.
+  iIntros "HQ Hh".
+  unfold own_heap.
+  iDestruct "Hh" as (H) "[Hh HH]".
+  iDestruct "Hh" as %Hh.
+  apply consume_sound with (1:=Hh) in Hconsume.
+  destruct Hconsume as (h' & env' & tree' & H1 & H2 & HH & Ha & Hh' & HQsymex).
+  iApply ("HQ" with "[% //]").
+  subst H.
+  iDestruct (own_logheap_lh_comp_elim with "HH") as "[HH1 HH2]".
+  iSplitL "HH1". {
+    unfold own_asn.
+    iExists H1.
+    iSplitL "". {
+      iPureIntro.
+      assumption.
+    }
+    iAssumption.
+  }
+  unfold own_heap.
+  iExists H2.
+  iSplitL "". {
+    iPureIntro.
+    assumption.
+  }
+  iAssumption.
+Qed.
+
+Lemma forall_ty_sound trace ty Q v:
+  forall_ty trace ty Q →
+  value_has_ty ty v →
+  Q v.
+Proof.
+  intros Hforall Hhas; destruct ty; try tauto; simpl in *; inversion Hhas; subst; auto.
+Qed.
+
+Definition spec_holds
+    (spec: Spec)(targs: list GenericArg)(args: list Value)
+    (wp_call: (Value → iProp Σ) → iProp Σ)
+    : iProp Σ :=
+  (* ⌜ values_have_tys (map snd (spec_params spec)) args ⌝ -∗ *)
+  let env := combine (map fst (spec_params spec)) (map (fun v => LSValue (Some v)) args) in
+  ∀ env',
+  own_asn env (pre spec) env' -∗
+  ∀ Q,
+  (∀ result,
+   ⌜ value_has_ty (spec_output spec) result ⌝ ∗
+   (∃ env'', own_asn (("result", LSValue (Some result))::env') (post spec) env'') -∗
+   Q result) -∗
+  wp_call Q.
+
+Definition spec_sound
+    (func_name: string)(targs: list GenericArg)(args: list Value)
+    (wp_call: string → list GenericArg → list Value → (Value → iProp Σ) → iProp Σ)
+    : iProp Σ :=
+  match assoc func_name specs with
+    None => True
+  | Some spec => spec_holds spec targs args (wp_call func_name targs args)
+  end.
+
+Lemma verify_call_sound trace h tree func_name targs args Qsymex wp_call Q:
+  verify_call specs trace h tree func_name targs args Qsymex →
+  (∀ h tree v, ⌜ Qsymex h tree v ⌝ -∗ own_heap h -∗ Q v) -∗
+  (∀ func_name targs args, spec_sound func_name targs args wp_call) -∗
+  own_heap h -∗
+  wp_call_std wp_call func_name targs args Q.
+Proof.
+  intros Hverify.
+  iIntros "HQ Hspecs Hh".
+  unfold wp_call_std.
+  unfold verify_call in Hverify.
+  destruct (string_dec func_name "std::ptr::mut_ptr::<impl *mut T>::is_null"). {
+    (* func_name = "std::ptr::mut_ptr::<impl *mut T>::is_null" *)
+    destruct args as [|arg [|]]; try tauto.
+    iApply ("HQ" with "[% //] Hh").
+  }
+  destruct (string_dec func_name "std::ptr::null_mut"). {
+    (* func_name = "std::ptr::null_mut" *)
+    iApply ("HQ" with "[% //] Hh").
+  }
+  destruct (string_dec func_name "std::process::abort"). {
+    (* func_name = "std::process:abort" *)
+    iPureIntro.
+    tauto.
+  }
+  iDestruct ("Hspecs" $! func_name targs args) as "Hspec".
+  unfold spec_sound.
+  destruct (assoc func_name specs); try tauto.
+  eapply consume_sound in Hverify.
+  iApply (Hverify with "[HQ Hspec] Hh").
+  iIntros (h' env' tree') "%Hforall".
+  iIntros "[Hpre Hh']".
+  iDestruct ("Hspec" $! env' with "Hpre") as "Hpost".
+  iApply "Hpost".
+  iIntros (result) "[Hresult Hpost]".
+  iDestruct "Hresult" as %Hresult.
+  iDestruct "Hpost" as (env'') "Hpost".
+  apply forall_ty_sound with (2:=Hresult) in Hforall.
+  iRevert "Hh' Hpost".
+  iApply produce_sound; try eassumption.
+  iIntros (h'' tree'').
+  iApply "HQ".
+Qed.
+
+Lemma consume_chunk_sound trace h tree Qsymex Q:
+  consume_chunk trace h tree Qsymex →
+  (∀ h tree chunk,
+   ⌜ Qsymex h tree chunk ⌝ -∗
+   own_heap h -∗ own_chunk chunk -∗ Q) -∗
+  own_heap h -∗ Q.
+Proof.
+  intros Hconsume.
+  iIntros "HQ Hh".
+  unfold own_heap.
+  iDestruct "Hh" as (H) "[Hh HH]".
+  iDestruct "Hh" as %Hh.
+  apply consume_chunk_sound with (1:=Hh) in Hconsume.
+  destruct Hconsume as (Hchunk & H' & h' & tree' & chunk & HH & HHchunk & Hh' & HQsymex).
+  iDestruct ("HQ" with "[% //]") as "HQ".
+  subst H.
+  iDestruct (own_logheap_lh_comp_elim with "HH") as "[HHchunk HH']".
+  iApply ("HQ" with "[HH'] [HHchunk]").
+  - unfold own_heap.
+    iExists H'.
+    iSplitL "". {
+      iPureIntro. assumption.
+    }
+    iAssumption.
+  - unfold own_chunk.
+    iExists Hchunk.
+    iSplitL "". {
+      iPureIntro. assumption.
+    }
+    iAssumption.
+Qed.
+
+Lemma eval_pats_sound trace env pats Qsymex:
+  eval_pats trace env pats Qsymex →
+  ∃ vs, Qsymex vs.
+Proof.
+  revert trace env Qsymex.
+  induction pats as [|pat pats]; intros trace env Qsymex; simpl.
+  - (* nil *)
+    intro HQsymex.
+    exists [].
+    assumption.
+  - (* cons *)
+    destruct pat.
+    + (* LitPat *)
+      intros Hpats.
+      apply IHpats in Hpats.
+      destruct Hpats as [vs Hpats].
+      exists (eval env e::vs).
+      assumption.
+    + (* VarPat *)
+      intros; tauto.
+Qed.
+
+Lemma verify_ghost_command_sound trace h env tree Qsymex Q:
+  verify_ghost_command preds trace h env tree Qsymex →
+  (∀ h tree, ⌜ Qsymex h tree ⌝ -∗ own_heap h -∗ Q) -∗
+  own_heap h -∗ Q.
+Proof.
+  iIntros (Hverify) "HQ".
+  destruct tree; try tauto.
+  destruct data; try tauto; simpl in Hverify.
+  - (* Open *)
+    iApply consume_chunk_sound; try eassumption.
+    clear Hverify.
+    iIntros (h' tree' chunk) "%Hchunk".
+    destruct chunk; try tauto.
+    case_eq (assoc pred_name preds). {
+      intros pred_def Hpred_name.
+      rewrite Hpred_name in Hchunk.
+      iIntros "Hh' Hchunk".
+      unfold own_chunk.
+      iDestruct "Hchunk" as (H) "[Hchunk HH]".
+      iDestruct "Hchunk" as %Hchunk'.
+      simpl in Hchunk'.
+      rewrite Hpred_name in Hchunk'.
+      destruct pred_def.
+      simpl in Hchunk.
+      destruct (combine_ params args) as [env' [[] []]]; try tauto.
+      destruct Hchunk' as [env'' Hbody].
+      iApply (produce_sound with "[HQ] Hh' [HH]").
+      - eassumption.
+      - iAssumption.
+      - unfold own_asn.
+        iExists H.
+        iSplitL "". {
+          iPureIntro. eassumption.
+        }
+        iAssumption.
+    }
+    intro Hpred_name.
+    rewrite Hpred_name in Hchunk.
+    tauto.
+  - (* Close *)
+    destruct coef; try tauto.
+    destruct q; try tauto.
+    destruct Qnum; try tauto.
+    destruct p; try tauto.
+    destruct Qden; try tauto.
+    destruct targs; try tauto.
+    apply eval_pats_sound in Hverify.
+    destruct Hverify as [vs Hverify].
+    case_eq (assoc pred_name preds). 2:{
+      intros Hpred_name.
+      rewrite Hpred_name in Hverify.
+      tauto.
+    }
+    intros pred_def Hpred_name.
+    rewrite Hpred_name in Hverify.
+    case_eq (combine_ (params pred_def) vs); intros env' [l l'] Hcombine_.
+    rewrite Hcombine_ in Hverify.
+    destruct l; try tauto.
+    destruct l'; try tauto.
+    iApply consume_sound; try eassumption.
+    iIntros (h' env'' tree') "%HQsymex".
+    iDestruct ("HQ" with "[% //]") as "HQ".
+    iIntros "[Hbody Hh']".
+    iApply "HQ".
+    unfold own_heap, own_asn.
+    iDestruct "Hbody" as (Hbody) "[Hbody_holds HHbody]".
+    iDestruct "Hbody_holds" as %Hbody_holds.
+    iDestruct "Hh'" as (Hh') "[Hh' HHh']".
+    iDestruct "Hh'" as %HHh'.
+    iExists (Hbody ⋅ Hh').
+    iSplitL "". {
+      iPureIntro.
+      simpl.
+      exists Hbody.
+      exists Hh'.
+      split. reflexivity.
+      rewrite Hpred_name.
+      destruct pred_def.
+      rewrite Hcombine_.
+      split. eexists; eassumption.
+      assumption.
+    }
+    iApply own_logheap_lh_comp_intro.
+    iFrame.
+Qed.
+
+Lemma verify_terminator_sound trace h env tree terminator Qsymex_return Qsymex_bb wp_call Qbb Qreturn:
+  verify_terminator preds specs local_decls trace h env tree terminator Qsymex_return Qsymex_bb →
+  (∀ h env tree, ⌜ Qsymex_return h env tree ⌝ -∗ own_heap h -∗ own_env Γ env -∗ Qreturn) -∗
+  ▷ (∀ func_name targs args, spec_sound func_name targs args wp_call) -∗
+  ▷ (∀ h env tree bb,
+     ⌜ Qsymex_bb h env tree bb ⌝ -∗
+     (∀ h env tree, ⌜ Qsymex_return h env tree ⌝ -∗ own_heap h -∗ own_env Γ env -∗ Qreturn) -∗
+     own_heap h -∗ own_env Γ env -∗ Qbb bb) -∗
+  own_heap h -∗
+  own_env Γ env -∗
+  wp_Terminator Γ terminator (wp_call_std wp_call) Qbb Qreturn.
+Proof.
+  intros Hverify.
+  iIntros "Hreturn Hspecs HQbb Hh Henv".
+  destruct terminator; simpl in Hverify.
+  - (* Goto *)
+    iApply wp_Goto_intro.
+    iNext.
+    iApply ("HQbb" $! h env tree target with "[% //] Hreturn Hh Henv").
+  - (* SwitchInt *)
+    iApply wp_SwitchInt_intro.
+    iApply (verify_operand_sound with "[Hreturn Hspecs HQbb] Hh Henv"); try eassumption.
+    clear Hverify.
+    iIntros (h0 tree0 v ty) "%Hverify Hh Henv".
+    iApply verify_switch_int_sound; try eassumption.
+    iNext.
+    iIntros (tree1 bb) "HQsymex_bb".
+    iApply ("HQbb" with "HQsymex_bb Hreturn Hh Henv").
+  - (* Return *)
+    iApply wp_Return_intro.
+    iApply ("Hreturn" with "[% //] Hh Henv").
+  - (* Unreachable *)
+    tauto.
+  - (* Call *)
+    destruct call.
+    destruct func; try tauto.
+    destruct const; try tauto.
+    destruct value; try tauto.
+    destruct ty; try tauto.
+    rename id into name.
+    destruct (string_dec name "VeriFast_ghost_command").
+    + (* name = "VeriFast_ghost_command" *)
+      subst.
+      iApply (verify_ghost_command_sound with "[Hreturn Hspecs HQbb Henv] Hh"); try eassumption.
+      clear Hverify.
+      iIntros (h0 tree0) "%Hverify Hh0".
+      simpl in Hverify.
+      destruct target; try tauto.
+      iApply wp_ghost_command_intro.
+      iNext.
+      iApply ("HQbb" with "[% //] Hreturn Hh0 Henv").
+    + (* name ≠ "VeriFast_ghost_command" *)
+      iApply wp_Call_intro.
+      iApply (verify_operands_sound with "[Hreturn Hspecs HQbb] Hh Henv"); try eassumption.
+      clear Hverify.
+      iIntros (h0 tree0 vs) "%Hverify Hh0 Henv".
+      iNext.
+      iApply (verify_call_sound with "[Hreturn HQbb Henv] Hspecs Hh0"); try eassumption.
+      clear Hverify.
+      iIntros (h1 tree1 v) "%Hverify Hh1".
+      iApply (verify_place_expr_sound with "[Hreturn HQbb] Hh1 Henv"); try eassumption.
+      clear Hverify.
+      iIntros (h2 tree2 place ty) "%Hverify %Hplace Hh2 Henv".
+      iDestruct (store_to_place_sound with "[Hreturn HQbb] Hh2 Henv") as "Hstore"; try eassumption. 2: {
+        iDestruct "Hstore" as "[Hpoints_to HQ]".
+        iDestruct "Hpoints_to" as (v0) "Hpoints_to".
+        iExists v0.
+        iFrame.
+      }
+      clear Hverify.
+      iIntros (h3 env0 tree3) "%Hverify Hh3 Henv0".
+      simpl in Hverify.
+      destruct target; try tauto.
+      iNext.
+      iApply ("HQbb" with "[% //] Hreturn Hh3 Henv0").
+Qed.
+
+Lemma verify_basic_block_sound trace h env tree bb Qsymex_return Qsymex_bb wp_call Qbb Qreturn:
+  verify_basic_block preds specs local_decls trace h env tree bb Qsymex_return Qsymex_bb →
+  (∀ h env tree, ⌜ Qsymex_return h env tree ⌝ -∗ own_heap h -∗ own_env Γ env -∗ Qreturn) -∗
+  ▷ (∀ func_name targs args, spec_sound func_name targs args wp_call) -∗
+  ▷ (∀ h env tree bb,
+     ⌜ Qsymex_bb h env tree bb ⌝ -∗
+     (∀ h env tree, ⌜ Qsymex_return h env tree ⌝ -∗ own_heap h -∗ own_env Γ env -∗ Qreturn) -∗
+     own_heap h -∗ own_env Γ env -∗ Qbb bb) -∗
+  own_heap h -∗
+  own_env Γ env -∗
+  wp_BasicBlock Γ bb (wp_call_std wp_call) Qbb Qreturn.
+Proof.
+  iIntros (Hverify) "Hreturn Hspecs Hbb Hh Henv".
+  unfold verify_basic_block in Hverify.
+  unfold wp_BasicBlock.
+  iApply (verify_statements_sound with "[Hreturn Hspecs Hbb] Hh Henv"); try eassumption.
+  clear Hverify.
+  iIntros (h0 env0 tree0) "%Hverify Hh0 Henv".
+  iApply (verify_terminator_sound with "Hreturn Hspecs Hbb Hh0 Henv"); eassumption.
+Qed.
+
+Lemma verify_basic_blocks_sound trace basic_blocks fuel h env tree bb Qsymex_return wp_call Qreturn:
+  verify_basic_blocks preds specs local_decls trace basic_blocks fuel h env tree bb Qsymex_return →
+  (∀ h env tree, ⌜ Qsymex_return h env tree ⌝ -∗ own_heap h -∗ own_env Γ env -∗ Qreturn) -∗
+  □ ▷ (∀ func_name targs args, spec_sound func_name targs args wp_call) -∗
+  own_heap h -∗
+  own_env Γ env -∗
+  wp_BasicBlocks Γ basic_blocks bb (wp_call_std wp_call) Qreturn.
+Proof.
+  revert trace h env tree bb.
+  induction fuel as [|fuel].
+  - (* O *)
+    intros trace h env tree bb Hverify.
+    tauto.
+  - (* S fuel *)
+    intros trace h env tree bb Hverify.
+    iIntros "Hreturn #Hspecs Hh Henv".
+    iApply wp_BasicBlocks_intro.
+    simpl in Hverify.
+    iApply (verify_basic_block_sound with "Hreturn Hspecs [] Hh Henv"); try eassumption.
+    clear Hverify.
+    iNext.
+    iIntros (h0 env0 tree0 bb0) "%Hverify Hreturn Hh0 Henv0".
+    destruct (assoc bb0 basic_blocks) as [bb'|]; try tauto.
+    iApply (IHfuel with "Hreturn Hspecs Hh0 Henv0"); try eassumption.
+Qed.
+
+End local_decls.
+
+Lemma alloc_params_sound trace h tree param_env Qsymex Q:
+  Forall (λ '((x, info), arg), ty info = (Γ x).1) param_env →
+  alloc_params trace h tree param_env Qsymex →
+  (∀ h env tree dealloc_params,
+   ⌜ Qsymex h env tree dealloc_params ⌝ -∗
+   (∀ trace h env tree Qsymex Q,
+    ⌜ dealloc_params trace h env tree Qsymex ⌝ -∗
+    (∀ h tree,
+     ⌜ Qsymex h tree ⌝ -∗
+     own_heap h -∗
+     Q) -∗
+    own_heap h -∗
+    own_env Γ env -∗
+    ([∗ list] '((x, {| ty := ty |}), _) ∈ param_env, ∃ state, points_to_ ty (VPtr (Γ x).2) state) ∗
+    Q) -∗
+   own_heap h -∗
+   own_env Γ env -∗
+   Q) -∗
+  own_heap h -∗
+  ([∗ list] '((x, {| ty := ty |}), v) ∈ param_env, points_to ty (VPtr (Γ x).2) v) -∗
+  Q.
+Proof.
+  revert trace h tree Qsymex Q.
+  induction param_env as [|[[x info] arg] param_env]; simpl.
+  - (* nil *)
+    iIntros (trace h tree Qsymex Q HΓ Halloc) "HQ Hh Hparam_env".
+    iApply ("HQ" with "[% //] [] Hh []").
+    + iIntros (_ h0 env tree0 Qsymex0 Q0) "%HQsymex0 HQ0 Hh0 Henv".
+      iSplitL "". done.
+      iApply ("HQ0" with "[% //] Hh0").
+    + simpl.
+      done.
+  - (* cons *)
+    iIntros (trace h etree Qsymex Q HΓ Halloc).
+    inversion HΓ; subst.
+    clear HΓ.
+    rename H1 into Hty_info.
+    rename H2 into HΓ.
+    destruct etree; try tauto.
+    destruct data; try tauto.
+    destruct (string_dec x0 x); try tauto.
+    subst.
+    iIntros "HQ Hh".
+    destruct info.
+    iIntros "[Hx Hparam_env]".
+    destruct addr_taken; try tauto.
+    iApply (IHparam_env with "[HQ Hx] Hh Hparam_env"); try eassumption.
+    iIntros (h0 env tree dealloc_params0) "%HQsymex Hdealloc_params0 Hh0 Henv".
+    iApply ("HQ" with "[% //] [Hdealloc_params0] Hh0 [Hx Henv]").
+    + iIntros (trace0 h1 env0 tree0 Qsymex0 Q0) "%Hdealloc HQ0 Hh1 Henv0".
+      case_eq (remove1_assoc x env0). 2:{
+        intros Hx; rewrite Hx in Hdealloc; tauto.
+      }
+      intros [xstate env1] Hx.
+      rewrite Hx in Hdealloc.
+      destruct xstate; try tauto.
+      iDestruct (remove1_assoc_own_env with "Henv0") as "[Hx Henv1]"; try eassumption.
+      rewrite <- Hty_info.
+      iFrame.
+      iApply ("Hdealloc_params0" with "[% //] HQ0 Hh1 Henv1").
+    + simpl.
+      rewrite <- Hty_info.
+      iFrame.
+Qed.
+
+Lemma alloc_locals_sound trace h env tree local_decls Qsymex Q:
+  Forall (λ '(x, info), ty info = (Γ x).1) local_decls →
+  alloc_locals trace h env tree local_decls Qsymex →
+  (∀ h env tree dealloc_locals,
+   ⌜ Qsymex h env tree dealloc_locals ⌝ -∗
+   (∀ trace h env tree Qsymex Q,
+    ⌜ dealloc_locals trace h env tree Qsymex ⌝ -∗
+    (∀ h env tree,
+     ⌜ Qsymex h env tree ⌝ -∗
+     own_heap h -∗
+     own_env Γ env -∗
+     Q) -∗
+    own_heap h -∗
+    own_env Γ env -∗
+    ([∗ list] '(x, {| ty := ty |}) ∈ local_decls, ∃ state, points_to_ ty (VPtr (Γ x).2) state) ∗
+    Q) -∗
+   own_heap h -∗
+   own_env Γ env -∗
+   Q) -∗
+  own_heap h -∗
+  own_env Γ env -∗
+  ([∗ list] '(x, {| ty := ty |}) ∈ local_decls, ∃ state, points_to_ ty (VPtr (Γ x).2) state) -∗
+  Q.
+Proof.
+  revert trace h env tree Qsymex Q.
+  induction local_decls as [|[x info] local_decls]; simpl.
+  - (* nil *)
+    iIntros (trace h env tree Qsymex Q _ Halloc) "HQ Hh Henv _".
+    iApply ("HQ" with "[% //] [] Hh Henv").
+    iIntros (trace0 h0 env0 tree0 Qsymex0 Q0) "%HQsymex0 HQ0 Hh0 Henv0".
+    iSplitL "". done.
+    iApply ("HQ0" with "[% //] Hh0 Henv0").
+  - (* cons *)
+    iIntros (trace h env tree Qsymex Q HΓ Halloc) "HQ Hh Henv [Hx Hlocal_decls]".
+    inversion HΓ; subst.
+    clear HΓ.
+    destruct info.
+    simpl in H1.
+    rename H1 into Hty.
+    rename H2 into HΓ.
+    destruct tree; try tauto.
+    destruct data; try tauto.
+    destruct (string_dec x x0); try tauto.
+    subst x0.
+    destruct addr_taken.
+    + (* true *)
+      destruct (Ty_eqb ty Never || Ty_eqb ty Tuple0).
+      * (* true *)
+        pose proof (Halloc':=Halloc (Γ x).2 VDummy (Γ_non_null x)).
+        iApply (IHlocal_decls with "[HQ Hx] Hh [Henv] Hlocal_decls"); try eassumption. 2:{
+          simpl.
+          iFrame.
+          done.
+        }
+        iIntros (h0 env0 tree0 dealloc_locals) "%HQsymex Hdealloc_locals_sound Hh0 Henv0".
+        iApply ("HQ" with "[% //] [Hdealloc_locals_sound Hx] Hh0 Henv0").
+        iIntros (trace0 h1 env1 tree1 Qsymex0 Q0) "%Hdealloc_locals HQ0 Hh1 Henv1".
+        iFrame.
+        iApply ("Hdealloc_locals_sound" with "[% //] [HQ0] Hh1 Henv1").
+        iAssumption.
+      * (* false *)
+        iDestruct "Hx" as (state) "Hx".
+        pose proof (Halloc':=Halloc (Γ x).2 state (Γ_non_null x)).
+        iApply (IHlocal_decls with "[HQ] [Hx Hh] [Henv] Hlocal_decls"); try eassumption.
+        2:{
+          iApply (own_heap_cons_intro with "[Hx] Hh").
+          iApply (own_chunk_prim_intro).
+          done.
+        }
+        2:{
+          simpl.
+          iSplitL "". done.
+          done.
+        }
+        iIntros (h0 env0 tree0 dealloc_locals) "%HQsymex Hdealloc_locals_sound Hh0 Henv0".
+        iApply ("HQ" with "[% //] [Hdealloc_locals_sound] Hh0 Henv0").
+        iIntros (trace0 h1 env1 tree1 Qsymex0 Q0) "%Hconsume HQ0 Hh1 Henv1".
+        assert (Hex: ∀ P (Q R: iProp Σ), (∃ (v: Value), P v ∗ Q ∗ R) -∗ ((∃ v, P v) ∗ Q) ∗ R). {
+          iIntros (P Q1 R) "[%v [HP [HQ HR]]]".
+          iSplitR "HR". {
+            iSplitR "HQ". {
+              iExists v.
+              done.
+            }
+            done.
+          }
+          done.
+        }
+        iApply Hex.
+        iApply (consume_points_to__sound with "[Hdealloc_locals_sound HQ0 Henv1] Hh1"); try eassumption.
+        iIntros (h2 tree2 v) "%Hdealloc Hh2".
+        iApply ("Hdealloc_locals_sound" with "[% //] [HQ0] Hh2 Henv1").
+        iAssumption.
+    + (* false *)
+      iApply (IHlocal_decls with "[HQ] Hh [Hx Henv] Hlocal_decls"); try eassumption. 2:{
+        rewrite Hty.
+        simpl. iFrame.
+      }
+      iIntros (h0 env0 tree0 dealloc_locals) "%HQsymex Hdealloc_locals_sound Hh0 Henv0".
+      iApply ("HQ" with "[% //] [Hdealloc_locals_sound] Hh0 Henv0").
+      iIntros (trace0 h1 env1 tree1 Qsymex0 Q0) "%Hdealloc HQ0 Hh1 Henv1".
+      case_eq (remove1_assoc x env1). 2:{
+        intros Hx; rewrite Hx in Hdealloc; tauto.
+      }
+      intros [xstate env2] Hx.
+      rewrite Hx in Hdealloc.
+      destruct xstate; try tauto.
+      iDestruct (remove1_assoc_own_env with "Henv1") as "[Hx Henv2]"; try eassumption.
+      rewrite Hty.
+      iFrame.
+      iApply ("Hdealloc_locals_sound" with "[% //] HQ0 Hh1 Henv2").
+Qed.
+
+End Γ.
+
+Lemma verify_body_sound trace h tree body args Qsymex wp_call Q:
+  verify_body preds specs trace h tree body args Qsymex →
+  □ ▷ (∀ func_name targs args, spec_sound func_name targs args wp_call) -∗
+  (∀ h tree result,
+   ⌜ Qsymex h tree result ⌝ -∗
+   own_heap h -∗
+   Q result) -∗
+  own_heap h -∗
+  wp_Body body args (wp_call_std wp_call) Q.
+Proof.
+  iIntros (Hverify) "#Hspecs HQ Hh".
+  unfold verify_body in Hverify.
+  unfold wp_Body.
+  iIntros (Γ) "%Γ_well_typed %Γ_non_null %Hlocal_decls_unique".
+  case_eq (local_decls body). {
+    intros Hlocal_decls.
+    rewrite Hlocal_decls in Hverify.
+    tauto.
+  }
+  intros [result_var result_var_info] local_decls' Hlocal_decls.
+  rewrite {1}Hlocal_decls in Hverify.
+  case_eq (combine_ local_decls' args).
+  intros param_env [local_decls'' args'] Hcombine_.
+  rewrite Hcombine_ in Hverify.
+  destruct (combine__append local_decls' args param_env local_decls'' args' Hcombine_) as [Hcombine_1 Hcombine_2].
+  subst.
+  iApply (alloc_params_sound with "[HQ] Hh"); try eassumption. {
+    rewrite Hlocal_decls in Hlocal_decls_unique.
+    apply Forall_cons_1 in Hlocal_decls_unique.
+    destruct Hlocal_decls_unique as [_ Hlocal_decls'_unique].
+    apply Forall_app in Hlocal_decls'_unique.
+    destruct Hlocal_decls'_unique as [H1 H2].
+    apply Forall_map in H1.
+    apply Forall_impl with (2:=H1).
+    intros.
+    destruct a.
+    simpl in H.
+    destruct p.
+    apply Γ_well_typed.
+    rewrite Hlocal_decls.
+    apply H.
+  }
+  clear Hverify.
+  iIntros (h0 env0 tree0 dealloc_params) "%Halloc_locals Hdealloc_params_sound Hh0 Henv0".
+  iApply (alloc_locals_sound with "[Hdealloc_params_sound HQ] Hh0 Henv0"); try eassumption. {
+    rewrite Hlocal_decls in Hlocal_decls_unique.
+    apply Forall_cons_1 in Hlocal_decls_unique.
+    destruct Hlocal_decls_unique as [Hresult_var_unique Hlocal_decls'_unique].
+    apply Forall_app in Hlocal_decls'_unique.
+    destruct Hlocal_decls'_unique as [Hparams_unique Hlocal_decls''_unique].
+    apply Forall_cons. {
+      apply Γ_well_typed.
+      rewrite Hlocal_decls.
+      assumption.
+    }
+    apply Forall_impl with (2:=Hlocal_decls''_unique).
+    intros [x info] Hx.
+    apply Γ_well_typed.
+    rewrite Hlocal_decls.
+    apply Hx.
+  }
+  clear Halloc_locals.
+  iIntros (h1 env tree1 dealloc_locals) "%Hverify_bb Hdealloc_locals_sound Hh1 Henv".
+  case_eq (basic_blocks body). {
+    intros Hbasic_blocks.
+    rewrite Hbasic_blocks in Hverify_bb.
+    tauto.
+  }
+  intros [bb0 bb_data0] basic_blocks' Hbasic_blocks.
+  rewrite <- Hbasic_blocks.
+  rewrite {1}Hbasic_blocks in Hverify_bb.
+  iApply (verify_basic_blocks_sound with "[-Hh1 Henv] Hspecs Hh1 Henv"); try eassumption.
+  clear Hverify_bb.
+  iIntros (h2 env1 tree2) "%Hverify_operand Hh2 Henv1".
+  iApply (verify_operand_sound with "[-Hh2 Henv1] Hh2 Henv1"); try eassumption.
+  iIntros (h3 tree3 result result_ty) "%Hdealloc_locals Hh3 Henv1".
+  iApply ("Hdealloc_locals_sound" with "[% //] [-Hh3 Henv1] Hh3 Henv1").
+  iIntros (h4 env2 tree4) "%Hdealloc_params Hh4 Henv2".
+  iApply ("Hdealloc_params_sound" with "[% //] [-Hh4 Henv2] Hh4 Henv2").
+  iIntros (h5 tree5) "%HQsymex Hh5".
+  iApply ("HQ" with "[% //] Hh5").
+Qed.
+
+Lemma forall_tys_sound trace tys Q vs:
+  forall_tys trace tys Q →
+  values_have_tys tys vs → Q vs.
+Proof.
+  revert trace Q vs.
+  induction tys as [|ty tys]; intros trace Q vs Hforall Hvs; destruct vs; simpl in *; try tauto.
+  destruct Hvs as [Hv Hvs].
+  apply forall_ty_sound with (v:=v) (2:=Hv) in Hforall.
+  apply IHtys with (1:=Hforall) (2:=Hvs).
+Qed.
+
+Lemma own_heap_nil:
+  ⊢ own_heap [].
+Proof.
+  unfold own_heap.
+  iExists ∅.
+  iSplitL "". {
+    iPureIntro.
+    unfold heap_holds.
+    reflexivity.
+  }
+  unfold own_logheap.
+  iApply lh_big_ast_lh_empty_intro.
+Qed.
+
+Lemma body_is_correct_sound trace body spec tree wp_call:
+  body_is_correct preds specs trace body spec tree →
+  □ ▷ (∀ func_name targs args, spec_sound func_name targs args wp_call) -∗
+  ∀ targs args,
+  spec_holds spec targs args (wp_Body' body args (wp_call_std wp_call)).
+Proof.
+  iIntros (Hcorrect) "#Hspecs %targs %args".
+  unfold body_is_correct in Hcorrect.
+  destruct (list_eq_dec Ty_eq_dec (map snd (spec_params spec)) (inputs body)) as [Hinputs|Hinputs]. 2:{
+    tauto.
+  }
+  destruct (Ty_eq_dec (spec_output spec) (output body)) as [Houtput|Houtput]. 2:{
+    tauto.
+  }
+  unfold spec_holds.
+  iIntros (env') "Hpre %Q HQ".
+  unfold wp_Body'.
+  iIntros "%Hvalues_have_tys".
+  rewrite {1}Hinputs in Hcorrect.
+  apply forall_tys_sound with (2:=Hvalues_have_tys) in Hcorrect.
+  iApply (produce_sound with "[HQ] [] Hpre"); try eassumption. 2:{
+    iApply own_heap_nil.
+  }
+  iIntros (h tree0) "%Hverify Hh".
+  iApply (verify_body_sound with "Hspecs [HQ] Hh"); try eassumption.
+  iIntros (h0 tree1 result) "%Hconsume Hh0".
+  iApply (consume_sound with "[HQ] Hh0"); try eassumption.
+  iIntros (h1 env'0 tree2) "_ [Hpost Hh1] %Hresult".
+  iApply ("HQ" with "[Hpost]").
+  iSplitL "". {
+    iPureIntro.
+    rewrite Houtput.
+    done.
+  }
+  iExists env'0.
+  iFrame.
+Qed.
+
+Lemma spec_holds_mono spec targs args wp_call wp_call':
+  (∀ Q, wp_call Q ⊢ wp_call' Q) →
+  spec_holds spec targs args wp_call ⊢
+  spec_holds spec targs args wp_call'.
+Proof.
+  intro Hwp_call.
+  iStartProof.
+  iIntros "Hholds".
+  unfold spec_holds.
+  iIntros "%Γ Hpre %Q HQ".
+  iApply Hwp_call.
+  iApply ("Hholds" with "Hpre HQ").
+Qed.
+
+Lemma spec_holds_True spec targs args:
+  ⊢ spec_holds spec targs args (λ result, True%I).
+Proof.
+  unfold spec_holds.
+  iIntros "%Γ Hpre %Q HQ".
+  done.
+Qed.
+
+Lemma bodies_are_correct_assoc trees bodies func_name body:
+  bodies_are_correct preds specs trees bodies →
+  assoc func_name bodies = Some body →
+  named_body_is_correct preds specs trees func_name body.
+Proof.
+  revert trees func_name body.
+  induction bodies as [|[func_name0 body0] bodies]; simpl; intros trees func_name body Hcorrect Hfunc_name.
+  - (* nil *)
+    discriminate.
+  - (* cons *)
+    destruct Hcorrect as [Hcorrect0 Hcorrect].
+    destruct (string_dec func_name func_name0).
+    + (* func_name = func_name0 *)
+      injection Hfunc_name; clear Hfunc_name; intros; subst.
+      assumption.
+    + (* func_name ≠ func_name0 *)
+      apply IHbodies with (1:=Hcorrect) (2:=Hfunc_name).
+Qed.
+
+Lemma bodies_are_correct_sound trees program:
+  bodies_are_correct preds specs trees program →
+  ⊢ □ (∀ func_name targs args, spec_sound func_name targs args (wp_Program program)).
+Proof.
+  intro Hcorrect.
+  iStartProof.
+  iLöb as "IH".
+  iModIntro.
+  iIntros (func_name targs args).
+  unfold spec_sound at 2.
+  case_eq (assoc func_name specs). 2:{
+    done.
+  }
+  intros spec Hspec.
+  iApply spec_holds_mono. {
+    intro Q.
+    iIntros "HQ".
+    iApply (wp_Program_intro with "HQ").
+  }
+  case_eq (assoc func_name program). 2:{
+    intro Hfunc_name.
+    iApply spec_holds_True.
+  }
+  intros body Hfunc_name.
+  apply bodies_are_correct_assoc with (2:=Hfunc_name) in Hcorrect.
+  unfold named_body_is_correct in Hcorrect.
+  rewrite Hspec in Hcorrect.
+  destruct (assoc_ ProofObligation_eq_dec (Verifying func_name) trees). 2:{
+    tauto.
+  }
+  iApply (body_is_correct_sound with "[IH]"); try eassumption.
+  iModIntro.
+  iNext.
+  iAssumption.
+Qed.
+
+End specs.
+
+End preds.
+
+End gfunctors.
+
+Theorem verified_program_has_no_ub preds specs trees program:
+  bodies_are_correct preds specs trees program →
+  assoc "main" specs = Some {|
+    spec_params := [];
+    spec_output := Tuple0;
+    pre := BoolAsn (BoolLit true);
+    post := BoolAsn (BoolLit true)
+  |} →
+  program_has_no_ub (Σ:=#[]) program.
+Proof.
+  intros Hcorrect Hmain.
+  unfold program_has_no_ub.
+  apply (bodies_are_correct_sound (Σ:=#[])) in Hcorrect.
+  unfold spec_sound in Hcorrect.
+  iDestruct Hcorrect as "#Hcorrect".
+  iSpecialize ("Hcorrect" $! "main" [] []).
+  rewrite Hmain.
+  unfold spec_holds.
+  simpl.
+  iSpecialize ("Hcorrect" $! [] with "[]"). {
+    unfold own_asn.
+    iExists ∅.
+    iSplitL "". {
+      iPureIntro.
+      constructor; done.
+    }
+    iApply own_logheap_lh_empty_intro.
+  }
+  iApply ("Hcorrect" with "[]").
+  iIntros "%result [%Hresult Hpost]".
+  done.
+Qed.
