bin/rust/rocq/Values.v
@@ -1,0 +1,82 @@
+From Coq Require Export QArith.
+
+Parameter Ptr: Set.
+
+Parameter null_ptr: Ptr.
+
+Parameter Ptr_eq_dec: forall (ptr1 ptr2: Ptr), {ptr1 = ptr2} + {ptr1 <> ptr2}.
+
+Inductive Value :=
+| VPtr(ptr: Ptr)
+| VBool(b: bool)
+| VReal(q: Q)
+| VDummy (* Used as the value of nonsensical expressions *)
+| VSome(v: Value)
+| VTuple0
+.
+
+Definition value_eq_dec(v1 v2: Value): {v1 = v2} + {v1 <> v2}.
+Admitted.
+
+Definition value_eqb(v1 v2: Value): bool.
+Admitted.
+
+Lemma value_eqb_def_(v1 v2: Value): (VBool (value_eqb v1 v2) = VBool true) = (v1 = v2).
+Admitted.
+
+From Coq Require Export List String.
+Import ListNotations.
+
+Fixpoint assoc{T}(x: string)(xys: list (string * T)): option T :=
+  match xys with
+    [] => None
+  | (x', y)::xys =>
+    if string_dec x x' then
+      Some y
+    else
+      assoc x xys
+  end.
+
+Fixpoint combine_{A B}(xs: list A)(ys: list B): list (A * B) * (list A * list B) :=
+  match xs, ys with
+    [], ys => ([], ([], ys))
+  | xs, [] => ([], (xs, []))
+  | (x::xs), (y::ys) =>
+    let '(xys, (xs, ys)) := combine_ xs ys in
+    ((x, y)::xys, (xs, ys))
+  end.
+
+Lemma combine__append{A B}(xs: list A)(ys: list B) xys xs' ys':
+  combine_ xs ys = (xys, (xs', ys')) ->
+  xs = map fst xys ++ xs' /\
+  ys = map snd xys ++ ys'.
+Proof.
+  revert ys xys xs' ys'.
+  induction xs; simpl; intros ys zys xs' ys'.
+  - (* nil *)
+    intros.
+    injection H; clear H; intros; subst.
+    split. {
+      reflexivity.
+    }
+    reflexivity.
+  - (* cons *)
+    destruct ys as [|y ys].
+    + intros.
+      injection H; clear H; intros; subst.
+      split. {
+        reflexivity.
+      }
+      reflexivity.
+    + case_eq (combine_ xs ys).
+      intros xys' [xs'' ys''] Hcombine_.
+      apply IHxs in Hcombine_.
+      destruct Hcombine_.
+      subst.
+      intros.
+      injection H; clear H; intros; subst.
+      split. {
+        reflexivity.
+      }
+      reflexivity.
+Qed.
